linearize cache

Impl/CacheImpl.i.dfy
@@ -1,5 +1,14 @@
 include "../lib/Base/DebugAccumulator.i.dfy"
+include "../lib/Base/sequences.i.dfy"
+include "../lib/Lang/LinearBox.i.dfy"
+include "../lib/Lang/LinearBox.s.dfy"
+include "../lib/Lang/LinearSequence.i.dfy"
+include "../lib/DataStructures/LinearContentMutableMap.i.dfy"
+include "../PivotBetree/Bounds.i.dfy"
 include "NodeImpl.i.dfy"
+include "BucketGeneratorImpl.i.dfy"
+include "FlushPolicyModel.i.dfy"
+
 //
 // Implements map<Reference, Node>
 //
@@ -9,7 +18,9 @@ include "NodeImpl.i.dfy"
 
 module CacheImpl {
   import DebugAccumulator
-  import opened BoxNodeImpl
+  import opened NodeImpl
+  import opened Bounds
+  import opened Sequences
   import opened Options
   import opened Maps
   import opened NativeTypes
@@ -17,77 +28,50 @@ module CacheImpl {
   import opened BucketWeights
   import opened KeyType
   import opened ValueMessage
+
   import BT = PivotBetreeSpec`Internal
   import Pivots = BoundedPivotsLib
+  import BucketsLib
 
-  // TODO(travis): it's ugly that we have to wrap this in a new object type
-  // just to have a Repr field. It also sucks that we have to have a Repr field
-  // at all instead of an opaque Repr() function, see
-  // https://github.com/dafny-lang/dafny/issues/377
-  // (jonh) but now that this file is next in line for the linearization
-  // steamroller, maybe don't sweat it.
-  class MutCache
-  {
-    var cache: MM.ResizingHashMap<Node>;
-    ghost var Repr: set<object>;
+  import BGI = BucketGeneratorImpl
+  import FPM = FlushPolicyModel
 
-    method DebugAccumulate()
-    returns (acc:DebugAccumulator.DebugAccumulator)
+  import opened LinearBox
+  import opened LinearBox_s
+  import opened LinearSequence_i
+  import opened LCMM = LinearContentMutableMap
+
+  linear datatype LMutCache = LMutCache(linear cache: LinearHashMap<Node>) {
+    static method DebugAccumulate(shared c: LMutCache)
+    returns (acc: DebugAccumulator.DebugAccumulator)
     requires false
     {
       acc := DebugAccumulator.EmptyAccumulator();
-      var a := new DebugAccumulator.AccRec(cache.Count, "Node");
+      var a := new DebugAccumulator.AccRec(c.cache.count, "Node");
       acc := DebugAccumulator.AccPut(acc, "cache", a);
     }
 
-    constructor()
-    ensures Inv();
-    ensures I() == map[]
-    ensures fresh(Repr);
+    static method NewCache() returns (linear newcache: LMutCache)
+    ensures newcache.Inv()
+    ensures newcache.I() == map[]
     {
-      cache := new MM.ResizingHashMap(128);
-      new;
-      Repr := {this} + cache.Repr + MutCacheBucketRepr();
+      linear var cache := LCMM.Constructor(128);
+      newcache := LMutCache(cache);
+    }
+    
+    predicate Inv()
+    {
+      && LCMM.Inv(cache)
+      && (forall ref | ref in cache.contents :: cache.contents[ref].Inv())
     }
 
-    protected function MutCacheBucketRepr() : set<object>
-    reads this, cache
-    reads set ref | ref in cache.Contents :: cache.Contents[ref]
-    {
-      set ref, o | ref in cache.Contents && o in cache.Contents[ref].Repr :: o
-    }
-
-    protected predicate CacheReprDisjoint(contents: map<BT.G.Reference, Node>)
-    reads set ref | ref in contents :: contents[ref]
-    {
-      forall ref1, ref2 | ref1 in contents && ref2 in contents && 
-          ref1 != ref2 :: contents[ref1].Repr !! contents[ref2].Repr
-    }
-
-    protected predicate Inv()
-    reads this, Repr
-    ensures Inv() ==> this in Repr
-    {
-      && cache in Repr
-      && (forall ref | ref in cache.Contents :: cache.Contents[ref] in Repr)
-      && Repr == {this} + cache.Repr + MutCacheBucketRepr()
-      && CacheReprDisjoint(cache.Contents)
-      && (forall ref | ref in cache.Contents :: cache.Contents[ref].Repr !! cache.Repr)
-      && (forall ref | ref in cache.Contents :: this !in cache.Contents[ref].Repr)
-      && this !in cache.Repr
-      && cache.Inv()
-      && (forall ref | ref in cache.Contents :: cache.Contents[ref].Inv()) // unhappy
-    }
-
-    protected function I() : map<BT.G.Reference, BT.G.Node>
-    reads this, Repr
+    function I() : map<BT.G.Reference, BT.G.Node>
     requires Inv()
     {
-      map ref | ref in cache.Contents :: cache.Contents[ref].I()
+      map ref | ref in cache.contents :: cache.contents[ref].I()
     }
 
-    protected function ptr(ref: BT.G.Reference) : Option<Node>
-    reads Repr
+    function ptr(ref: BT.G.Reference) : Option<Node>
     requires Inv()
     ensures ptr(ref).None? ==> ref !in I()
     ensures ptr(ref).Some? ==>
@@ -95,185 +79,771 @@ module CacheImpl {
         && ptr(ref).value.Inv()
         && I()[ref] == ptr(ref).value.I()
     {
-      if ref in cache.Contents then Some(cache.Contents[ref]) else None
+      if ref in cache.contents then Some(cache.contents[ref]) else None
     }
 
-    method GetOpt(ref: BT.G.Reference)
-    returns (node: Option<Node>)
+    shared method InCache(ref: BT.G.Reference) returns (b: bool)
     requires Inv()
-    ensures node == ptr(ref)
+    ensures b == ptr(ref).Some?
     {
-      node := cache.Get(ref);
+      b := IsEntry(cache.underlying, ref);
     }
 
-    lemma LemmaNodeReprLeRepr(ref: BT.G.Reference)
+    shared method Get(ref: BT.G.Reference)
+    returns (shared node: Node)
     requires Inv()
-    ensures ptr(ref).Some? ==> ptr(ref).value.Repr <= Repr
+    requires ptr(ref).Some?
+    ensures node == ptr(ref).value
     {
+      node := LCMM.Get(cache, ref);
     }
 
     lemma LemmaSizeEqCount()
     requires Inv()
-    ensures |I()| == |cache.Contents|
+    ensures |I()| == |cache.contents|
     {
-      assert I().Keys == cache.Contents.Keys;
+      assert I().Keys == cache.contents.Keys;
       assert |I()|
           == |I().Keys|
-          == |cache.Contents.Keys|
-          == |cache.Contents|;
+          == |cache.contents.Keys|
+          == |cache.contents|;
     }
 
-    protected function method Count() : (c : uint64)
-    reads this, Repr
-    requires Inv()
-    ensures c as int == |I()|
+    linear inout method Insert(ref: BT.G.Reference, linear node: Node)
+    requires old_self.Inv()
+    requires node.Inv()
+    requires |old_self.I()| <= 0x10000
+    ensures self.Inv()
+    ensures self.I() == old_self.I()[ref := node.I()]
+    ensures forall r | r != ref :: self.ptr(r) == old_self.ptr(r)
     {
-      LemmaSizeEqCount();
-      cache.Count
+      self.LemmaSizeEqCount(); 
+      linear var replaced := LCMM.Insert(inout self.cache, ref, node);
+      linear match replaced {
+        case lSome(oldnode) => {
+          var _ := FreeNode(oldnode);
+        }
+        case lNone() => { }
+      }
+      assert self.cache.contents[ref] == node;
+      assert self.Inv();
     }
 
-    method Insert(ref: BT.G.Reference, node: Node)
+    linear inout method ReplaceAndGet(ref: BT.G.Reference, linear newNode: Node)
+    returns (linear oldNode: Node)
+    requires old_self.Inv()
+    requires old_self.ptr(ref).Some?
+    requires |old_self.I()| <= 0x10000
+    requires newNode.Inv()
+    ensures self.Inv()
+    ensures oldNode.Inv()
+    ensures |self.I()| == |old_self.I()|
+    ensures oldNode == old_self.ptr(ref).value
+    ensures self.I() == old_self.I()[ref := newNode.I()]
+    ensures forall r | r != ref :: self.ptr(r) == old_self.ptr(r)
+    {
+      self.LemmaSizeEqCount();
+
+      linear var replaced := LCMM.Insert(inout self.cache, ref, newNode);
+      assert replaced.lSome?;
+      linear var lSome(node) := replaced;
+      oldNode := node;
+
+      assert self.cache.contents[ref] == newNode;
+      assert self.Inv();
+
+      self.LemmaSizeEqCount();
+    }
+
+    linear inout method RemoveAndGet(ref: BT.G.Reference) returns (linear node: Node)
+    requires old_self.Inv()
+    requires old_self.ptr(ref).Some?
+    ensures self.Inv()
+    ensures node.Inv()
+    ensures node == old_self.ptr(ref).value
+    ensures self.I() == MapRemove1(old_self.I(), ref)
+    {
+      self.LemmaSizeEqCount();
+      linear var removed := LCMM.Remove(inout self.cache, ref);
+      assert removed.lSome?;
+      linear var lSome(value) := removed;
+      node := value;
+      assert self.Inv();
+    }
+
+    linear inout method Remove(ref: BT.G.Reference)
+    requires old_self.Inv()
+    ensures self.Inv()
+    ensures self.I() == MapRemove1(old_self.I(), ref)
+    {
+      self.LemmaSizeEqCount();
+      linear var removed := LCMM.Remove(inout self.cache, ref);
+      linear match removed {
+        case lSome(node) => {
+          assert node.Inv();
+          var _ := FreeNode(node);
+        }
+        case lNone() => { }
+      }
+      assert self.Inv();
+    }
+
+    // This is used for the 'grow' operation.
+    linear inout method MoveAndReplace(oldref: BT.G.Reference,
+      newref: BT.G.Reference, linear node: Node)
+    requires old_self.Inv()
+    requires node.Inv()
+    requires |old_self.I()| <= 0x10000
+    requires oldref in old_self.I()
+    ensures self.Inv()
+    ensures self.I() == old_self.I()[oldref := node.I()][newref := old_self.I()[oldref]]
+    {
+      self.LemmaSizeEqCount();
+      linear var replaced := LCMM.Insert(inout self.cache, oldref, node);
+      assert self.cache.contents[oldref] == node;
+      assert replaced.lSome?;
+
+      linear var lSome(oldnode) := replaced;
+      linear var replaced2 := LCMM.Insert(inout self.cache, newref, oldnode);
+      linear match replaced2 {
+        case lSome(n) => {
+          var _ := FreeNode(n);
+        }
+        case lNone() => { }
+      }
+    }
+
+    // Like Insert, but with slightly different requires
+    linear inout method Overwrite(ref: BT.G.Reference, linear node: Node)
+    requires old_self.Inv()
+    requires node.Inv()
+    requires ref in old_self.I()
+    requires |old_self.I()| <= 0x10000
+    ensures self.Inv()
+    ensures self.I() == old_self.I()[ref := node.I()]
+    {
+      Insert(inout self, ref, node);
+    }
+
+    linear inout method NodeUpdateSlot(ref: BT.G.Reference, slot: uint64, 
+      linear bucket: MutBucket, childref: BT.G.Reference)
+    returns (newchildren: Option<seq<BT.G.Reference>>)
+    requires old_self.Inv()
+    requires bucket.Inv()
+    requires old_self.ptr(ref).Some?
+    requires BT.WFNode(old_self.I()[ref])
+    requires |old_self.I()| <= 0x10000
+    requires old_self.I()[ref].children.Some?
+    requires slot as int + 1 < 0x1_0000_0000_0000_0000
+    requires slot as nat < |old_self.I()[ref].children.value|
+    ensures self.Inv()
+    ensures self.I() == old_self.I()[ref := BT.G.Node(
+        old_self.I()[ref].pivotTable,
+        Some(old_self.I()[ref].children.value[slot as int := childref]),
+        old_self.I()[ref].buckets[slot as int := bucket.bucket]
+      )]
+    ensures newchildren == self.I()[ref].children
+    {
+      linear var node := inout self.RemoveAndGet(ref);
+      inout node.UpdateSlot(slot, bucket, childref);
+      newchildren := node.children;
+      inout self.Insert(ref, node);
+    }
+
+    linear inout method InsertKeyValue(ref: BT.G.Reference, key: Key, msg: Message)
+    requires old_self.Inv()
+    requires old_self.ptr(ref).Some?
+    requires |old_self.I()| <= 0x10000
+    requires BT.WFNode(old_self.I()[ref])
+    requires Pivots.BoundedKey(old_self.I()[ref].pivotTable, key)
+    requires WeightBucketList(old_self.I()[ref].buckets) + WeightKey(key) 
+      + WeightMessage(msg) < 0x1_0000_0000_0000_0000
+    ensures self.Inv()
+    ensures self.I() == old_self.I()
+      [ref := BT.NodeInsertKeyValue(old_self.I()[ref], key, msg)]
+    {
+      linear var node := inout self.RemoveAndGet(ref);
+      inout node.InsertKeyValue(key, msg);
+      inout self.Insert(ref, node);
+    }
+
+    linear inout method SplitParent(ref: BT.G.Reference, slot: uint64, pivot: Key,
+      left_childref: BT.G.Reference, right_childref: BT.G.Reference)
+    requires old_self.Inv()
+    requires old_self.ptr(ref).Some?
+    requires BT.WFNode(old_self.I()[ref])
+    requires old_self.I()[ref].children.Some?
+    requires 0 <= slot as int < |old_self.I()[ref].children.value|
+    requires 0 <= slot as int < |old_self.I()[ref].buckets|
+    requires |old_self.I()| <= 0x10000
+    ensures self.Inv()
+    ensures self.I() == old_self.I()[ref := BT.SplitParent(old_self.I()[ref],
+      pivot, slot as int, left_childref, right_childref)]
+    {
+      linear var node := inout self.RemoveAndGet(ref);
+      inout node.SplitParent(slot, pivot, left_childref, right_childref);
+      inout self.Insert(ref, node);
+    }
+
+    /// Temporary node borrow methods
+
+    shared method GetNodeInfo(ref: BT.G.Reference)
+    returns (pivots: Pivots.PivotTable, children: Option<seq<BT.G.Reference>>)
+    requires Inv()
+    requires ptr(ref).Some?
+    ensures pivots == I()[ref].pivotTable
+    ensures children == I()[ref].children
+    {
+      shared var node := Get(ref);
+      children := node.children;
+      pivots := node.pivotTable;
+    }
+
+    shared method GetNodeBucketsLen(ref: BT.G.Reference)
+    returns (len: uint64)
+    requires Inv()
+    requires ptr(ref).Some?
+    ensures len as nat == |I()[ref].buckets|
+    {
+      shared var node := Get(ref);
+      len := lseq_length_as_uint64(node.buckets);
+    }
+
+    shared method GetMessage(ref: BT.G.Reference, i: uint64, key: KeyType.Key)
+    returns (msg: Option<Message>)
+    requires Inv()
+    requires ptr(ref).Some?
+    requires BT.WFNode(I()[ref])
+    requires Pivots.BoundedKey(I()[ref].pivotTable, key)
+    requires i as int == Pivots.Route(I()[ref].pivotTable, key)
+    ensures 
+      && var bucket := I()[ref].buckets[i];
+      && msg == BucketsLib.bucketBinarySearchLookup(bucket, key)
+    {
+      shared var node := Get(ref);
+      msg := lseq_peek(node.buckets, i).Query(key);
+    }
+
+    shared method NodeBucketsWeight(ref: BT.G.Reference)
+    returns (weight: uint64)
+    requires Inv()
+    requires ptr(ref).Some?
+    requires BT.WFNode(I()[ref])
+    ensures weight as int == WeightBucketList(I()[ref].buckets)
+    {
+      shared var node := Get(ref);
+      weight := MutBucket.computeWeightOfSeq(node.buckets);
+    }
+
+    shared method NodeBoundedBucket(ref: BT.G.Reference, 
+      pivotsref: BT.G.Reference, slot: uint64)
+    returns (b: bool)
+    requires Inv()
+    requires ref in I()
+    requires pivotsref in I()
+    requires BT.WFNode(I()[ref])
+    requires BT.WFNode(I()[pivotsref])
+    requires slot as nat < |I()[ref].buckets|
+    ensures b == Pivots.BoundedKeySeq(I()[pivotsref].pivotTable,
+        I()[ref].buckets[slot as nat].keys)
+    {
+      shared var node := Get(ref);
+      if ref == pivotsref {
+        b := node.BoundedBucket(node.pivotTable, slot);
+      } else {
+        shared var pivotsnode := Get(pivotsref);
+        b := node.BoundedBucket(pivotsnode.pivotTable, slot);
+      }
+    }
+
+    shared method NodePartialFlush(parentref: BT.G.Reference, 
+      childref: BT.G.Reference, slot: uint64)
+    returns (linear newparentBucket: MutBucket, linear newchild: Node)
+    requires Inv()
+    requires parentref in I()
+    requires childref in I()
+    requires BT.WFNode(I()[parentref])
+    requires BT.WFNode(I()[childref])
+    requires slot as nat < |I()[parentref].buckets|
+    ensures newparentBucket.Inv()
+    ensures newchild.Inv()
+    ensures newchild.I().pivotTable == I()[childref].pivotTable
+    ensures newchild.I().children == I()[childref].children
+    ensures BucketModel.partialFlushResult(newparentBucket.I(), newchild.I().buckets)
+        == BucketModel.partialFlush(I()[parentref].buckets[slot], 
+          I()[childref].pivotTable, I()[childref].buckets)
+    {
+      shared var parent := Get(parentref);
+      shared var child := Get(childref);
+
+      WeightBucketLeBucketList(parent.I().buckets, slot as int);
+      assert WeightBucketList(child.I().buckets) <= MaxTotalBucketWeight();
+
+      linear var newpbucket, newbuckets := BucketImpl.PartialFlush(
+        lseq_peek(parent.buckets, slot as uint64), child.buckets, child.pivotTable);
+
+      newchild := Node(child.pivotTable, child.children, newbuckets);
+      newparentBucket := newpbucket;
+    }
+
+    shared method NodeSplitMiddle(ref: BT.G.Reference)
+    returns (linear left: MutBucket, linear right: MutBucket, pivot: Key)
+    requires Inv()
+    requires ref in I()
+    requires BT.WFNode(I()[ref])
+    requires |I()[ref].buckets| == 1
+    ensures left.Inv()
+    ensures right.Inv()
+    ensures
+      && var bucket := I()[ref].buckets[0];
+      && pivot == BucketsLib.getMiddleKey(bucket)
+      && left.I() == BucketsLib.SplitBucketLeft(bucket, pivot)
+      && right.I() == BucketsLib.SplitBucketRight(bucket, pivot)
+    {
+      shared var node := Get(ref);
+      shared var bucket := lseq_peek(node.buckets, 0);
+
+      pivot := bucket.GetMiddleKey(); 
+      left, right := MutBucket.SplitLeftRight(bucket, pivot);
+    }
+
+    shared method NodeCutOff(ref: BT.G.Reference, lbound: KeyType.Key, ubound: Option<KeyType.Key>)
+    returns (linear node': Node)
+    requires Inv()
+    requires ptr(ref).Some?
+    requires BT.WFNode(I()[ref])
+    requires BT.ValidSplitKey(I()[ref], lbound, ubound)
+    ensures node'.Inv()
+    ensures node'.I() == BT.CutoffNode(I()[ref], lbound, ubound)
+    {
+      shared var node := Get(ref);
+      node' := node.CutoffNode(lbound, ubound);
+    }
+
+    shared method NodeBucketGen(ref: BT.G.Reference, r: uint64, start: BT.UI.RangeStart)
+    returns (linear g: BGI.Generator)
+    requires Inv()
+    requires ptr(ref).Some?
+    requires BT.WFNode(I()[ref])
+    requires r as nat < |I()[ref].buckets|
+    ensures g.Basic?
+    ensures g.biter.bucket == I()[ref].buckets[r as nat]
+    ensures g.Inv()
+    ensures g.I() == BGI.BucketGeneratorModel.GenFromBucketWithLowerBound(
+        I()[ref].buckets[r as nat], start)
+    {
+      shared var node := Get(ref);
+      g := BGI.Generator.GenFromBucketWithLowerBound(
+          lseq_peek(node.buckets, r), start);
+    }
+
+    shared method NodeBiggestSlot(ref: BT.G.Reference)
+    returns (res : (uint64, uint64))
+    requires Inv()
+    requires ptr(ref).Some?
+    requires FPM.biggestSlot.requires(I()[ref].buckets)
+    ensures res == FPM.biggestSlot(I()[ref].buckets)
+    {
+      shared var node := Get(ref);
+      shared var buckets := node.buckets;
+
+      WeightBucketLeBucketList(MutBucket.ILseq(buckets), 0);
+      var j := 1;
+      var bestIdx := 0;
+      var bestWeight := lseq_peek(buckets, 0).weight;
+
+      while j < lseq_length_as_uint64(buckets)
+      invariant FPM.biggestSlotIterate.requires(MutBucket.ILseq(buckets), j, bestIdx, bestWeight)
+      invariant FPM.biggestSlotIterate(MutBucket.ILseq(buckets), j, bestIdx, bestWeight) 
+        == FPM.biggestSlot(MutBucket.ILseq(buckets))
+      {
+        WeightBucketLeBucketList(MutBucket.ILseq(buckets), j as int);
+        var w := lseq_peek(buckets, j).weight;
+        if w > bestWeight {
+          bestIdx := j;
+          bestWeight := w;
+        }
+        j := j + 1;
+      }
+      return (bestIdx, bestWeight);
+    }
+  }
+
+  function method CacheCount(shared cache: LMutCache) : (c : uint64)
+  requires cache.Inv()
+  ensures c as int == |cache.I()|
+  {
+    cache.LemmaSizeEqCount();
+    cache.cache.count
+  }
+
+  // boxed cache
+  // TODO(Jialin): switch to boxedoption
+  class MutCache {
+    var box: BoxedLinear<LMutCache>;
+    ghost var Repr: set<object>;
+
+    function Read() : LMutCache
+    requires box.Inv()
+    reads this, box, box.Repr
+    {
+      box.Read()
+    }
+
+    protected predicate Inv()
+    reads this, Repr
+    ensures Inv() ==> this in Repr
+    {
+      && box in Repr
+      && Repr == {this} + box.Repr
+      && box.Inv()
+      && box.Has()
+      && Read().Inv()
+    }
+
+    constructor ()
+    ensures Inv()
+    ensures I() == map[]
+    ensures fresh(Repr)
+    {
+      linear var cache := LMutCache.NewCache();
+      box := new BoxedLinear(cache);
+      new;
+      Repr := {this} + box.Repr;
+    }
+    
+    method DebugAccumulate()
+    returns (acc: DebugAccumulator.DebugAccumulator)
+    requires box.Inv()
+    requires box.Has()
+    requires false
+    {
+     acc := LMutCache.DebugAccumulate(box.Borrow());
+    }
+
+    protected function I() : map<BT.G.Reference, BT.G.Node>
+    requires Inv()
+    reads Repr
+    {
+      Read().I()
+    }
+
+    protected function ptr(ref: BT.G.Reference) : Option<Node>
+    requires Inv()
+    reads this, box, box.Repr
+    ensures ptr(ref).None? ==> ref !in I()
+    ensures ptr(ref).Some? ==>
+        && ref in I()
+        && ptr(ref).value.Inv()
+        && I()[ref] == ptr(ref).value.I()
+    {
+      Read().ptr(ref)
+    }
+
+    method InCache(ref: BT.G.Reference) returns (b: bool)
+    requires Inv()
+    ensures b == ptr(ref).Some?
+    {
+      b := this.box.Borrow().InCache(ref);
+    }
+
+    method Insert(ref: BT.G.Reference, linear node: Node)
     requires Inv()
     requires node.Inv()
-    requires Repr !! node.Repr
     requires |I()| <= 0x10000
-    modifies Repr
     ensures Inv()
     ensures I() == old(I()[ref := node.I()])
     ensures forall r | r != ref :: ptr(r) == old(ptr(r))
-    ensures forall o | o in Repr :: o in old(Repr) || o in old(node.Repr) || fresh(o)
+    ensures Repr == old(Repr)
+    modifies this.Repr
     {
-      LemmaSizeEqCount();
+      linear var c := this.box.Take();
+      inout c.Insert(ref, node);
+      this.box.Give(c);
+    }
 
-      cache.Insert(ref, node);
+    method ReplaceAndGet(ref: BT.G.Reference, linear newNode: Node)
+    returns (linear oldNode: Node)
+    requires Inv()
+    requires newNode.Inv()
+    requires ptr(ref).Some?
+    requires |I()| <= 0x10000
+    ensures Inv()
+    ensures oldNode.Inv()
+    ensures |I()| == |old(I())|
+    ensures oldNode == old(ptr(ref)).value
+    ensures I() == old(I())[ref := newNode.I()]
+    ensures forall r | r != ref :: ptr(r) == old(ptr(r))
+    ensures Repr == old(Repr)
+    modifies this.Repr
+    {
+      linear var c := this.box.Take();
+      oldNode := inout c.ReplaceAndGet(ref, newNode);
+      this.box.Give(c);
+    }
 
-      assert cache.Contents[ref] == node;
-      Repr := {this} + cache.Repr + MutCacheBucketRepr();
-
-      assert Inv();
+    method RemoveAndGet(ref: BT.G.Reference) returns (linear node: Node)
+    requires Inv()
+    requires ptr(ref).Some?
+    ensures Inv()
+    ensures node.Inv()
+    ensures node == old(ptr(ref)).value
+    ensures I() == MapRemove1(old(I()), ref)
+    ensures Repr == old(Repr)
+    modifies this.Repr
+    {
+      linear var c := this.box.Take();
+      node := inout c.RemoveAndGet(ref);
+      this.box.Give(c);
     }
 
     method Remove(ref: BT.G.Reference)
     requires Inv()
-    modifies Repr
     ensures Inv()
     ensures I() == MapRemove1(old(I()), ref)
-    ensures forall o | o in Repr :: o in old(Repr) || fresh(o)
+    ensures Repr == old(Repr)
+    modifies this.Repr
     {
-      LemmaSizeEqCount();
-      var _ := cache.RemoveAndGet(ref);
-      Repr := {this} + cache.Repr + MutCacheBucketRepr();
-
-      assert Inv();
+      linear var c := this.box.Take();
+      inout c.Remove(ref);
+      this.box.Give(c);
     }
 
     // This is used for the 'grow' operation.
-    method MoveAndReplace(oldref: BT.G.Reference, newref: BT.G.Reference, node: Node)
+    method MoveAndReplace(oldref: BT.G.Reference,
+      newref: BT.G.Reference, linear node: Node)
     requires Inv()
     requires node.Inv()
-    requires Repr !! node.Repr
     requires |I()| <= 0x10000
     requires oldref in I()
-    modifies Repr
     ensures Inv()
-    ensures I() == old(I()[newref := I()[oldref]][oldref := node.I()])
-    ensures forall o | o in Repr :: o in old(Repr) || o in old(node.Repr) || fresh(o)
+    ensures I() == old(I())[oldref := node.I()][newref := old(I())[oldref]]
+    ensures Repr == old(Repr)
+    modifies this.Repr
     {
-      LemmaSizeEqCount();
-      var oldnodeOpt := cache.Get(oldref);
-      var oldnode := oldnodeOpt.value;
-      cache.Insert(newref, oldnode);
-      cache.Insert(oldref, node);
-
-      Repr := {this} + cache.Repr + MutCacheBucketRepr();
-      assert Inv();
+      linear var c := this.box.Take();
+      inout c.MoveAndReplace(oldref, newref, node);
+      this.box.Give(c);
     }
 
     // Like Insert, but with slightly different requires
-    method Overwrite(ref: BT.G.Reference, node: Node)
+    method Overwrite(ref: BT.G.Reference, linear node: Node)
     requires Inv()
     requires node.Inv()
     requires ref in I()
-    requires forall o | o in node.Repr :: o in cache.Contents[ref].Repr || o !in Repr
     requires |I()| <= 0x10000
-    modifies Repr
     ensures Inv()
-    ensures I() == old(I()[ref := node.I()])
-    ensures forall o | o in Repr :: o in old(Repr) || o in old(node.Repr) || fresh(o)
+    ensures I() == old(I())[ref := node.I()]
+    ensures Repr == old(Repr)
+    modifies this.Repr
     {
-      LemmaSizeEqCount();
-      cache.Insert(ref, node);
-      assert cache.Contents[ref] == node;
-      Repr := {this} + cache.Repr + MutCacheBucketRepr();
-
-      assert Inv();
+      linear var c := this.box.Take();
+      inout c.Overwrite(ref, node);
+      this.box.Give(c);
     }
 
-    method UpdateNodeSlot(ghost ref: BT.G.Reference, node: Node, slot: uint64, linear bucket: MutBucket, childref: BT.G.Reference)
+    function method Count() : (c : uint64)
+    requires Inv()
+    reads this, Repr
+    ensures c as int == |I()|
+    {
+      CacheCount(this.box.Borrow())
+    }
+
+    method NodeUpdateSlot(ref: BT.G.Reference, slot: uint64, 
+      linear bucket: MutBucket, childref: BT.G.Reference)
+    returns (newchildren: Option<seq<BT.G.Reference>>)
     requires Inv()
     requires bucket.Inv()
-    requires ref in I()
-    requires I()[ref].children.Some?
-    requires 0 <= slot as int < |I()[ref].children.value|
-    requires 0 <= slot as int < |I()[ref].buckets|
-    requires slot as int + 1 < 0x1_0000_0000_0000_0000
+    requires ptr(ref).Some?
+    requires BT.WFNode(I()[ref])
     requires |I()| <= 0x10000
-    requires ptr(ref) == Some(node)
-    modifies Repr
+    requires I()[ref].children.Some?
+    requires slot as nat < |I()[ref].children.value|
+    requires slot as int + 1 < 0x1_0000_0000_0000_0000
     ensures Inv()
     ensures I() == old(I()[ref := BT.G.Node(
         I()[ref].pivotTable,
         Some(I()[ref].children.value[slot as int := childref]),
         I()[ref].buckets[slot as int := bucket.bucket]
       )])
-    ensures forall o | o in Repr :: o in old(Repr) || fresh(o)
+    ensures newchildren == I()[ref].children
+    ensures Repr == old(Repr)
+    modifies this.Repr
     {
-      //var nodeOpt := cache.Get(ref);
-      //var node := nodeOpt.value;
-      node.UpdateSlot(slot, bucket, childref);
-
-      Repr := {this} + cache.Repr + MutCacheBucketRepr(); 
-      assert Inv();
-    }
-
-    method SplitParent(ref: BT.G.Reference, slot: uint64, pivot: Key, left_childref: BT.G.Reference, right_childref: BT.G.Reference)
-    requires Inv()
-    requires ref in I()
-    requires BT.WFNode(I()[ref])
-    requires I()[ref].children.Some?
-    requires 0 <= slot as int < |I()[ref].children.value|
-    requires 0 <= slot as int < |I()[ref].buckets|
-    requires |I()| <= 0x10000
-    modifies Repr
-    ensures Inv()
-    ensures I() == old(I()[ref := BT.SplitParent(I()[ref], pivot, slot as int, left_childref, right_childref)])
-    ensures forall o | o in Repr :: o in old(Repr) || fresh(o)
-    {
-      var nodeOpt := GetOpt(ref);
-      var node := nodeOpt.value;
-      node.SplitParent(slot, pivot, left_childref, right_childref);
-
-      Repr := {this} + cache.Repr + MutCacheBucketRepr();
-      assert Inv();
+      linear var c := this.box.Take();
+      newchildren := inout c.NodeUpdateSlot(ref, slot, bucket, childref);
+      this.box.Give(c);
     }
 
     method InsertKeyValue(ref: BT.G.Reference, key: Key, msg: Message)
     requires Inv()
     requires ref in I()
+    requires ptr(ref).Some?
+    requires |I()| <= 0x10000
     requires BT.WFNode(I()[ref])
     requires Pivots.BoundedKey(I()[ref].pivotTable, key)
-    requires WeightBucketList(I()[ref].buckets) + WeightKey(key) + WeightMessage(msg) < 0x1_0000_0000_0000_0000
-    modifies Repr
+    requires WeightBucketList(I()[ref].buckets) + WeightKey(key) 
+      + WeightMessage(msg) < 0x1_0000_0000_0000_0000
     ensures Inv()
-    ensures I() == old(I())[ref := BT.NodeInsertKeyValue(old(I())[ref], key, msg)]
-    ensures forall o | o in Repr :: o in old(Repr) || fresh(o)
+    ensures I() == old(I()[ref := BT.NodeInsertKeyValue(I()[ref], key, msg)])
+    ensures Repr == old(Repr)
+    modifies this.Repr
     {
-      var nodeOpt := GetOpt(ref);
-      var node := nodeOpt.value;
-      node.InsertKeyValue(key, msg);
+      linear var c := this.box.Take();
+      inout c.InsertKeyValue(ref, key, msg);
+      this.box.Give(c);
+    }
 
-      Repr := {this} + cache.Repr + MutCacheBucketRepr();
-      assert Inv();
+    method SplitParent(ref: BT.G.Reference, slot: uint64, pivot: Key,
+      left_childref: BT.G.Reference, right_childref: BT.G.Reference)
+    requires Inv()
+    requires ptr(ref).Some?
+    requires BT.WFNode(I()[ref])
+    requires I()[ref].children.Some?
+    requires 0 <= slot as int < |I()[ref].children.value|
+    requires 0 <= slot as int < |I()[ref].buckets|
+    requires |I()| <= 0x10000
+    ensures Inv()
+    ensures I() == old(I()[ref := BT.SplitParent(I()[ref],
+      pivot, slot as int, left_childref, right_childref)])
+    ensures Repr == old(Repr)
+    modifies this.Repr
+    {
+      linear var c := this.box.Take();
+      inout c.SplitParent(ref, slot, pivot, left_childref, right_childref);
+      this.box.Give(c);
+    }
+
+    /// temporary node methods
+    method GetNodeInfo(ref: BT.G.Reference)
+    returns (pivots: Pivots.PivotTable, children: Option<seq<BT.G.Reference>>)
+    requires Inv()
+    requires ptr(ref).Some?
+    ensures pivots == I()[ref].pivotTable
+    ensures children == I()[ref].children
+    {
+      pivots, children := this.box.Borrow().GetNodeInfo(ref);
+    }
+
+    method GetNodeBucketsLen(ref: BT.G.Reference)
+    returns (len: uint64)
+    requires Inv()
+    requires ptr(ref).Some?
+    ensures len as nat == |I()[ref].buckets|
+    {
+      len := this.box.Borrow().GetNodeBucketsLen(ref);
+    }
+
+    method GetMessage(ref: BT.G.Reference, i: uint64, key: KeyType.Key)
+    returns (msg: Option<Message>)
+    requires Inv()
+    requires ptr(ref).Some?
+    requires BT.WFNode(I()[ref])
+    requires Pivots.BoundedKey(I()[ref].pivotTable, key)
+    requires i as int == Pivots.Route(I()[ref].pivotTable, key)
+    ensures 
+      && var bucket := I()[ref].buckets[i];
+      && msg == BucketsLib.bucketBinarySearchLookup(bucket, key)
+    {
+      msg := this.box.Borrow().GetMessage(ref, i, key);
+    }
+
+    method NodeBucketsWeight(ref: BT.G.Reference) returns (weight: uint64)
+    requires Inv()
+    requires ptr(ref).Some?
+    requires BT.WFNode(I()[ref])
+    ensures weight as int == WeightBucketList(I()[ref].buckets)
+    {
+      weight := this.box.Borrow().NodeBucketsWeight(ref);
+    }
+  
+    method NodeBoundedBucket(ref: BT.G.Reference, 
+      pivotsref: BT.G.Reference, slot: uint64) returns (b: bool)
+    requires Inv()
+    requires ref in I()
+    requires pivotsref in I()
+    requires BT.WFNode(I()[ref])
+    requires BT.WFNode(I()[pivotsref])
+    requires slot as nat < |I()[ref].buckets|
+    ensures b == Pivots.BoundedKeySeq(I()[pivotsref].pivotTable,
+        I()[ref].buckets[slot as nat].keys)
+    {
+      b := this.box.Borrow().NodeBoundedBucket(ref, pivotsref, slot);
+    }
+
+    method NodePartialFlush(parentref: BT.G.Reference, 
+      childref: BT.G.Reference, slot: uint64)
+    returns (linear newparentBucket: MutBucket, linear newchild: Node)
+    requires Inv()
+    requires parentref in I()
+    requires childref in I()
+    requires BT.WFNode(I()[parentref])
+    requires BT.WFNode(I()[childref])
+    requires slot as nat < |I()[parentref].buckets|
+    ensures newparentBucket.Inv()
+    ensures newchild.Inv()
+    ensures newchild.I().pivotTable == I()[childref].pivotTable
+    ensures newchild.I().children == I()[childref].children
+    ensures BucketModel.partialFlushResult(newparentBucket.I(), newchild.I().buckets)
+        == BucketModel.partialFlush(I()[parentref].buckets[slot],
+          I()[childref].pivotTable, I()[childref].buckets)
+    {
+      newparentBucket, newchild := this.box.Borrow().NodePartialFlush(parentref, childref, slot);
+    }
+
+    method NodeSplitMiddle(ref: BT.G.Reference)
+    returns (linear left: MutBucket, linear right: MutBucket, pivot: Key)
+    requires Inv()
+    requires ref in I()
+    requires BT.WFNode(I()[ref])
+    requires |I()[ref].buckets| == 1
+    ensures left.Inv()
+    ensures right.Inv()
+    ensures
+      && var bucket := I()[ref].buckets[0];
+      && pivot == BucketsLib.getMiddleKey(bucket)
+      && left.I() == BucketsLib.SplitBucketLeft(bucket, pivot)
+      && right.I() == BucketsLib.SplitBucketRight(bucket, pivot)
+    {
+      left, right, pivot := this.box.Borrow().NodeSplitMiddle(ref);
+    }
+
+    method NodeCutOff(ref: BT.G.Reference, lbound: KeyType.Key,ubound: Option<KeyType.Key>)
+    returns (linear node': Node)
+    requires Inv()
+    requires ptr(ref).Some?
+    requires BT.WFNode(I()[ref])
+    requires BT.ValidSplitKey(I()[ref], lbound, ubound)
+    ensures node'.Inv()
+    ensures node'.I() == BT.CutoffNode(I()[ref], lbound, ubound)
+    {
+      node' := this.box.Borrow().NodeCutOff(ref, lbound, ubound);
+    }
+
+    method NodeBucketGen(ref: BT.G.Reference, r: uint64, start: BT.UI.RangeStart)
+    returns (linear g: BGI.Generator)
+    requires Inv()
+    requires ptr(ref).Some?
+    requires BT.WFNode(I()[ref])
+    requires r as nat < |I()[ref].buckets|
+    ensures g.Basic?
+    ensures g.biter.bucket == I()[ref].buckets[r as nat]
+    ensures g.Inv()
+    ensures g.I() == BGI.BucketGeneratorModel.GenFromBucketWithLowerBound(
+        I()[ref].buckets[r as nat], start)
+    {
+      g := this.box.Borrow().NodeBucketGen(ref, r, start);
+    }
+
+    method NodeBiggestSlot(ref: BT.G.Reference)
+    returns (res : (uint64, uint64))
+    requires Inv()
+    requires ptr(ref).Some?
+    requires FPM.biggestSlot.requires(I()[ref].buckets)
+    ensures res == FPM.biggestSlot(I()[ref].buckets)
+    {
+      res := this.box.Borrow().NodeBiggestSlot(ref);
     }
   }
 }
