Impl/FlushPolicyImpl.i.dfy
@@ -29,32 +29,35 @@ module FlushPolicyImpl {
   import opened BucketsLib
   import opened BucketWeights
 
-  method biggestSlot(shared buckets: lseq<MutBucket>) returns (res : (uint64, uint64))
-  requires MutBucket.InvLseq(buckets)
-  requires FlushPolicyModel.biggestSlot.requires(MutBucket.ILseq(buckets))
-  ensures res == FlushPolicyModel.biggestSlot(old(MutBucket.ILseq(buckets)))
-  {
-    WeightBucketLeBucketList(MutBucket.ILseq(buckets), 0);
-    var j := 1;
-    var bestIdx := 0;
-    var bestWeight := lseq_peek(buckets, 0).weight;
+  // temporarily moving method to cache
+  // method biggestSlot(shared buckets: lseq<MutBucket>) returns (res : (uint64, uint64))
+  // requires MutBucket.InvLseq(buckets)
+  // requires FlushPolicyModel.biggestSlot.requires(MutBucket.ILseq(buckets))
+  // ensures res == FlushPolicyModel.biggestSlot(MutBucket.ILseq(buckets))
+  // {
+  //   WeightBucketLeBucketList(MutBucket.ILseq(buckets), 0);
+  //   var j := 1;
+  //   var bestIdx := 0;
+  //   var bestWeight := lseq_peek(buckets, 0).weight;
 
-    while j < lseq_length_raw(buckets)
-    invariant FlushPolicyModel.biggestSlotIterate.requires(MutBucket.ILseq(buckets), j, bestIdx, bestWeight)
-    invariant FlushPolicyModel.biggestSlotIterate(MutBucket.ILseq(buckets), j, bestIdx, bestWeight) == FlushPolicyModel.biggestSlot(MutBucket.ILseq(buckets))
-    {
-      WeightBucketLeBucketList(MutBucket.ILseq(buckets), j as int);
-      var w := lseq_peek(buckets, j).weight;
-      if w > bestWeight {
-        bestIdx := j;
-        bestWeight := w;
-      }
-      j := j + 1;
-    }
-    return (bestIdx, bestWeight);
-  }
+  //   while j < lseq_length_raw(buckets)
+  //   invariant FlushPolicyModel.biggestSlotIterate.requires(MutBucket.ILseq(buckets), j, bestIdx, bestWeight)
+  //   invariant FlushPolicyModel.biggestSlotIterate(MutBucket.ILseq(buckets), j, bestIdx, bestWeight) == FlushPolicyModel.biggestSlot(MutBucket.ILseq(buckets))
+  //   {
+  //     WeightBucketLeBucketList(MutBucket.ILseq(buckets), j as int);
+  //     var w := lseq_peek(buckets, j).weight;
+  //     if w > bestWeight {
+  //       bestIdx := j;
+  //       bestWeight := w;
+  //     }
+  //     j := j + 1;
+  //   }
+  //   return (bestIdx, bestWeight);
+  // }
 
-  method getActionToSplit(s: ImplVariables, stack: seq<BT.G.Reference>, slots: seq<uint64>, i: uint64) returns (action : FlushPolicyModel.Action)
+  method getActionToSplit(s: ImplVariables, stack: seq<BT.G.Reference>,
+    slots: seq<uint64>, i: uint64)
+  returns (action : FlushPolicyModel.Action)
   requires 0 <= i as int < |stack|
   requires Inv(s)
   requires FlushPolicyModel.ValidStackSlots(s.I(), stack, slots)
@@ -70,11 +73,9 @@ module FlushPolicyImpl {
         action := FlushPolicyModel.ActionEvict;
       }
     } else {
-      var nodePrev := s.cache.GetOpt(stack[i-1]);
-      var nodePrevChildren := nodePrev.value.GetChildren();
+      var _, nodePrevChildren := s.cache.GetNodeInfo(stack[i-1]);
       if |nodePrevChildren.value| as uint64 < MaxNumChildrenUint64() {
-        var nodeThis := s.cache.GetOpt(stack[i]);
-        var bucketslen := nodeThis.value.GetBucketsLen();
+        var bucketslen := s.cache.GetNodeBucketsLen(stack[i]);
         if bucketslen == 1 {
           action := FlushPolicyModel.ActionRepivot(stack[i]);
         } else {
@@ -90,7 +91,8 @@ module FlushPolicyImpl {
     }
   }
 
-  method getActionToFlush(s: ImplVariables, stack: seq<BT.G.Reference>, slots: seq<uint64>) returns (action : FlushPolicyModel.Action)
+  method getActionToFlush(s: ImplVariables, stack: seq<BT.G.Reference>, slots: seq<uint64>)
+  returns (action : FlushPolicyModel.Action)
   requires |stack| <= 40
   requires Inv(s)
   requires FlushPolicyModel.ValidStackSlots(s.I(), stack, slots)
@@ -106,29 +108,22 @@ module FlushPolicyImpl {
       action := FlushPolicyModel.ActionFail;
     } else {
       var ref := stack[|stack| as uint64 - 1];
-      var nodeOpt := s.cache.GetOpt(ref);
-      var node := nodeOpt.value;
-      var children := node.GetChildren();
-      var bucketslen := node.GetBucketsLen();
+      var _, children := s.cache.GetNodeInfo(ref);
+      var bucketslen := s.cache.GetNodeBucketsLen(ref);
 
       if children.None? || bucketslen == MaxNumChildrenUint64() {
         action := getActionToSplit(s, stack, slots, |stack| as uint64 - 1);
       } else {
-        var bs:(uint64, uint64) := biggestSlot(node.box.Borrow().buckets);
+        var bs:(uint64, uint64) := s.cache.NodeBiggestSlot(ref);
         var (slot, slotWeight) := bs;
         if bucketslen as uint64 < 8 {
           var childref := children.value[slot];
-          var childOpt := s.cache.GetOpt(childref);
-          if childOpt.Some? {
-            s.cache.LemmaNodeReprLeRepr(childref);
-            var child := childOpt.value;
-            assert MutBucket.InvLseq(child.Read().buckets);
+          var childincache := s.cache.InCache(childref);
+          if childincache {
             s.lru.Use(childref);
-            assert MutBucket.InvLseq(child.Read().buckets);
             LruModel.LruUse(old(s.lru.Queue), childref);
 
-            var childTotalWeight: uint64 := MutBucket.computeWeightOfSeq(child.box.Borrow().buckets);
-
+            var childTotalWeight := s.cache.NodeBucketsWeight(childref);
             if childTotalWeight + FlushTriggerWeightUint64() <= MaxTotalBucketWeightUint64() {
               if TotalCacheSize(s) <= MaxCacheSizeUint64() - 1 {
                 action := FlushPolicyModel.ActionFlush(ref, slot);
@@ -179,22 +174,16 @@ module FlushPolicyImpl {
         PageInNodeReq(s, io, ref);
       }
       case ActionSplit(parentref, slot) => {
-        var parent := s.cache.GetOpt(parentref);
-        var parent_children := parent.value.GetChildren();
+        var _, parent_children := s.cache.GetNodeInfo(parentref);
         doSplit(s, parentref, parent_children.value[slot], slot);
       }
       case ActionRepivot(ref) => {
-        var node := s.cache.GetOpt(ref);
-        repivotLeaf(s, ref, node.value);
+        repivotLeaf(s, ref);
       }
       case ActionFlush(parentref, slot) => {
-        var parent := s.cache.GetOpt(parentref);
-        var parent_children := parent.value.GetChildren();
+        var _, parent_children := s.cache.GetNodeInfo(parentref);
         var childref := parent_children.value[slot];
-        var child := s.cache.GetOpt(childref);
-        flush(s, parentref, slot, 
-            parent_children.value[slot],
-            child.value);
+        flush(s, parentref, slot, childref);
       }
       case ActionGrow => {
         grow(s);
