Impl/NodeImpl.i.dfy
@@ -18,6 +18,7 @@ module NodeImpl {
   import opened ValueMessage
 
   import BT = PivotBetreeSpec`Internal
+  import PivotBetree
   import Pivots = BoundedPivotsLib
   import PKV = PackedKV
   import opened Bounds
@@ -28,9 +29,15 @@ module NodeImpl {
   import MM = MutableMap
   import ReferenceType`Internal
 
-  linear datatype Node = Node(pivotTable: Pivots.PivotTable, children: Option<seq<BT.G.Reference>>, linear buckets: lseq<BucketImpl.MutBucket>)
+  linear datatype Node = Node(
+      pivotTable: Pivots.PivotTable, 
+      children: Option<seq<BT.G.Reference>>,
+      linear buckets: lseq<BucketImpl.MutBucket>)
   {
-    static method Alloc(pivotTable: Pivots.PivotTable, children: Option<seq<BT.G.Reference>>, linear buckets: lseq<BucketImpl.MutBucket>) returns (linear node: Node)
+    static method Alloc(pivotTable: Pivots.PivotTable, 
+      children: Option<seq<BT.G.Reference>>, 
+      linear buckets: lseq<BucketImpl.MutBucket>)
+    returns (linear node: Node)
     requires MutBucket.InvLseq(buckets)
     ensures node.pivotTable == pivotTable;
     ensures node.children == children;
@@ -52,37 +59,31 @@ module NodeImpl {
         BucketImpl.MutBucket.ILseq(buckets))
     }
 
-    static method GetBucketsLen(shared node: Node) returns (len: uint64)
-    requires node.Inv()
-    ensures len as nat == |node.buckets|
+    static method EmptyNode() returns (linear node: Node)
+    ensures node.Inv()
+    ensures node.I() == PivotBetree.EmptyNode()
+    ensures BT.WFNode(node.I())
     {
-      len := lseq_length_raw(node.buckets);
+      linear var mutbucket := MutBucket.Alloc();
+      linear var buckets := lseq_alloc(1);
+      lseq_give_inout(inout buckets, 0, mutbucket);
+      
+      node := Node(Pivots.InitPivotTable(), None, buckets);
+      assert node.I().buckets == [B(map[])];
+      WeightBucketListOneEmpty();
     }
 
-    static method GetChildren(shared node: Node) returns (children: Option<seq<BT.G.Reference>>)
-    requires node.Inv()
-    ensures children == node.children
-    {
-      children := node.children;
-    }
-
-    static method GetPivots(shared node: Node) returns (pivots: Pivots.PivotTable)
-    requires node.Inv()
-    ensures pivots == node.pivotTable
-    {
-      pivots := node.pivotTable;
-    }
-
-    static method BoundedBucket(shared node: Node, pivots: Pivots.PivotTable, slot: uint64) returns (result: bool)
-    requires node.Inv()
+    shared method BoundedBucket(pivots: Pivots.PivotTable, slot: uint64)
+    returns (result: bool)
+    requires Inv()
     requires |pivots| < 0x4000_0000_0000_0000
     requires Pivots.WFPivots(pivots)
-    requires slot as nat < |node.buckets|
-    ensures result == Pivots.BoundedKeySeq(pivots, node.buckets[slot as nat].I().keys)
+    requires slot as nat < |buckets|
+    ensures result == Pivots.BoundedKeySeq(pivots, buckets[slot as nat].I().keys)
     {
-      var pkv := lseq_peek(node.buckets, slot).GetPkv();
+      var pkv := lseq_peek(buckets, slot).GetPkv();
       ghost var keys := PKV.IKeys(pkv.keys);
-      assert node.buckets[slot as nat].I().keys == keys;
+      assert buckets[slot as nat].I().keys == keys;
 
       var bounded := true;
       var i := 0 as uint64;
@@ -108,26 +109,26 @@ module NodeImpl {
       result := lseq_peek(buckets, slot).WellMarshalled();
     }
 
-    static method BucketsWellMarshalled(shared node: Node) returns (result: bool)
-    requires node.Inv()
-    requires |node.buckets| < Uint64UpperBound()
-    ensures result == BucketsLib.BucketListWellMarshalled(MutBucket.ILseq(node.buckets))
+    shared method BucketsWellMarshalled() returns (result: bool)
+    requires Inv()
+    requires |buckets| < Uint64UpperBound()
+    ensures result == BucketsLib.BucketListWellMarshalled(MutBucket.ILseq(buckets))
     {
       var i: uint64 := 0;
 
-      while i < lseq_length_raw(node.buckets)
-        invariant i as nat <= |node.buckets|
-        invariant BucketListWellMarshalled(MutBucket.ISeq(lseqs(node.buckets)[..i]))
+      while i < lseq_length_raw(buckets)
+        invariant i as nat <= |buckets|
+        invariant BucketListWellMarshalled(MutBucket.ISeq(lseqs(buckets)[..i]))
       {
-        var bwm := lseq_peek(node.buckets, i).WellMarshalled();
+        var bwm := lseq_peek(buckets, i).WellMarshalled();
         
         if !bwm {
           return false;
         }
-        assert lseqs(node.buckets)[..i+1] == lseqs(node.buckets)[..i] + [ node.buckets[i as nat] ];
+        assert lseqs(buckets)[..i+1] == lseqs(buckets)[..i] + [ buckets[i as nat] ];
         i := i + 1;
       }
-      assert lseqs(node.buckets) == lseqs(node.buckets)[..i];
+      assert lseqs(buckets) == lseqs(buckets)[..i];
       return true;  
     }
 
@@ -173,12 +174,12 @@ module NodeImpl {
       assert a == b;
     }
 
-    shared method CutoffNodeAndKeepLeft(pivot: Key) returns (linear node': Node)
+    shared method CutoffNodeAndKeepLeft(pivot: Key) returns (linear node: Node)
     requires Inv()
     requires BT.WFNode(I())
     requires Pivots.ValidLeftCutOffKey(pivotTable, pivot)
-    ensures node'.Inv()
-    ensures node'.I() == BT.CutoffNodeAndKeepLeft(I(), pivot);
+    ensures node.Inv()
+    ensures node.I() == BT.CutoffNodeAndKeepLeft(I(), pivot);
     {
       BT.reveal_CutoffNodeAndKeepLeft();
       var cLeft := Pivots.ComputeCutoffForLeft(this.pivotTable, pivot);
@@ -189,15 +190,15 @@ module NodeImpl {
       linear var splitBucket := lseq_peek(buckets, cLeft).SplitLeft(pivot);
       linear var slice := MutBucket.CloneSeq(this.buckets, 0, cLeft); // TODO clone not necessary?
       linear var leftBuckets := InsertLSeq(slice, splitBucket, cLeft);
-      node' := Node(leftPivots, leftChildren, leftBuckets);
+      node := Node(leftPivots, leftChildren, leftBuckets);
     }
 
-    shared method CutoffNodeAndKeepRight(pivot: Key) returns (linear node': Node)
+    shared method CutoffNodeAndKeepRight(pivot: Key) returns (linear node: Node)
     requires Inv()
     requires BT.WFNode(I())
     requires Pivots.BoundedKey(pivotTable, pivot)
-    ensures node'.Inv()
-    ensures node'.I() == BT.CutoffNodeAndKeepRight(I(), pivot);
+    ensures node.Inv()
+    ensures node.I() == BT.CutoffNodeAndKeepRight(I(), pivot);
     {
       BT.reveal_CutoffNodeAndKeepRight();
       var cRight := Pivots.ComputeCutoffForRight(this.pivotTable, pivot);
@@ -208,64 +209,64 @@ module NodeImpl {
       linear var splitBucket := lseq_peek(buckets, cRight).SplitRight(pivot);
       linear var slice := MutBucket.CloneSeq(buckets, cRight + 1, lseq_length_raw(buckets));
       linear var rightBuckets := InsertLSeq(slice, splitBucket, 0);
-      node' := Node(rightPivots, rightChildren, rightBuckets);
-      assert node'.I().buckets == BT.CutoffNodeAndKeepRight(I(), pivot).buckets;
-      assert node'.I().children == BT.CutoffNodeAndKeepRight(I(), pivot).children;
-      assert node'.I().pivotTable == BT.CutoffNodeAndKeepRight(I(), pivot).pivotTable;
+      node := Node(rightPivots, rightChildren, rightBuckets);
+      assert node.I().buckets == BT.CutoffNodeAndKeepRight(I(), pivot).buckets;
+      assert node.I().children == BT.CutoffNodeAndKeepRight(I(), pivot).children;
+      assert node.I().pivotTable == BT.CutoffNodeAndKeepRight(I(), pivot).pivotTable;
     }
 
-    static method CutoffNode(shared node: Node, lbound: Key, rbound: Option<Key>)
-    returns (linear node' : Node)
-    requires node.Inv()
-    requires BT.WFNode(node.I())
-    requires BT.ValidSplitKey(node.I(), lbound, rbound)
-    ensures node'.Inv()
-    ensures node'.I() == BT.CutoffNode(node.I(), lbound, rbound)
+    shared method CutoffNode(lbound: Key, rbound: Option<Key>)
+    returns (linear node : Node)
+    requires Inv()
+    requires BT.WFNode(I())
+    requires BT.ValidSplitKey(I(), lbound, rbound)
+    ensures node.Inv()
+    ensures node.I() == BT.CutoffNode(I(), lbound, rbound)
     {
       BT.reveal_CutoffNode();
       match rbound {
         case None => {
-          node' := node.CutoffNodeAndKeepRight(lbound);
+          node := CutoffNodeAndKeepRight(lbound);
         }
         case Some(rbound) => {
-          linear var node1 := node.CutoffNodeAndKeepLeft(rbound);
-          node' := node1.CutoffNodeAndKeepRight(lbound);
+          linear var node1 := CutoffNodeAndKeepLeft(rbound);
+          node := node1.CutoffNodeAndKeepRight(lbound);
           var _ := FreeNode(node1);
         }
       }
     }
 
-    static method SplitChildLeft(shared node: Node, num_children_left: uint64)
-    returns (linear node': Node)
-    requires node.Inv()
-    requires |node.pivotTable| < Uint64UpperBound()
-    requires 0 <= num_children_left as int - 1 <= |node.pivotTable| - 2
-    requires node.children.Some? ==> 0 <= num_children_left as int <= |node.children.value|
-    requires 0 <= num_children_left as int <= |node.buckets|
-    ensures node'.Inv()
-    ensures node'.I() == BT.SplitChildLeft(node.I(), num_children_left as int)
+    shared method SplitChildLeft(num_children_left: uint64)
+    returns (linear node: Node)
+    requires Inv()
+    requires |pivotTable| < Uint64UpperBound()
+    requires 0 <= num_children_left as int - 1 <= |pivotTable| - 2
+    requires children.Some? ==> 0 <= num_children_left as int <= |children.value|
+    requires 0 <= num_children_left as int <= |buckets|
+    ensures node.Inv()
+    ensures node.I() == BT.SplitChildLeft(I(), num_children_left as int)
     {
-      linear var slice := MutBucket.CloneSeq(node.buckets, 0, num_children_left);
-      node' := Node(
-        node.pivotTable[ .. num_children_left + 1 ],
-        if node.children.Some? then Some(node.children.value[ .. num_children_left ]) else None,
+      linear var slice := MutBucket.CloneSeq(buckets, 0, num_children_left);
+      node := Node(
+        pivotTable[ .. num_children_left + 1 ],
+        if children.Some? then Some(children.value[ .. num_children_left ]) else None,
         slice
       );
     }
 
-    static method SplitChildRight(shared node: Node, num_children_left: uint64)
-    returns (linear node': Node)
-    requires node.Inv()
-    requires 0 <= num_children_left as int <= |node.pivotTable| - 1
-    requires node.children.Some? ==> 0 <= num_children_left as int <= |node.children.value|
-    requires 0 <= num_children_left as int <= |node.buckets|
-    ensures node'.Inv()
-    ensures node'.I() == BT.SplitChildRight(node.I(), num_children_left as int)
+    shared method SplitChildRight(num_children_left: uint64)
+    returns (linear node: Node)
+    requires Inv()
+    requires 0 <= num_children_left as int <= |pivotTable| - 1
+    requires children.Some? ==> 0 <= num_children_left as int <= |children.value|
+    requires 0 <= num_children_left as int <= |buckets|
+    ensures node.Inv()
+    ensures node.I() == BT.SplitChildRight(I(), num_children_left as int)
     {
-      linear var slice := MutBucket.CloneSeq(node.buckets, num_children_left, lseq_length_raw(node.buckets));
-      node' := Node(
-        node.pivotTable[ num_children_left .. ],
-        if node.children.Some? then Some(node.children.value[ num_children_left .. ]) else None,
+      linear var slice := MutBucket.CloneSeq(buckets, num_children_left, lseq_length_raw(buckets));
+      node := Node(
+        pivotTable[ num_children_left .. ],
+        if children.Some? then Some(children.value[ num_children_left .. ]) else None,
         slice
       );
     }
@@ -274,8 +275,9 @@ module NodeImpl {
     requires old_self.Inv();
     requires BT.WFNode(old_self.I())
     requires Pivots.BoundedKey(old_self.pivotTable, key)
-    requires WeightBucketList(MutBucket.ILseq(buckets)) + WeightKey(key) + WeightMessage(msg) < 0x1_0000_0000_0000_0000
-    ensures self.Inv();
+    requires WeightBucketList(MutBucket.ILseq(buckets)) + WeightKey(key) + WeightMessage(msg) 
+      < 0x1_0000_0000_0000_0000
+    ensures self.Inv()
     ensures self.I() == BT.NodeInsertKeyValue(old_self.I(), key, msg)
     {
       BT.reveal_NodeInsertKeyValue();
@@ -303,214 +305,5 @@ module NodeImpl {
   {
     linear var Node(_, _, buckets) := node;
     FreeMutBucketSeq(buckets)
-  }
-}
-
-// boxed linear node, use till we have linear mutable map with linear items
-module BoxNodeImpl {
-  import opened LinearSequence_s
-  import opened LinearSequence_i
-  import opened LinearBox_s
-  import opened LinearBox
-  import opened KeyType
-  import opened ValueMessage
-  import opened NativeTypes
-  import opened BucketImpl
-  import opened BucketWeights
-  import opened Options
-
-  import IM = StateModel
-  import MM = MutableMap
-  import BT = PivotBetreeSpec`Internal
-
-  import L : NodeImpl
-
-  class Node {
-    var box: BoxedLinearOption<L.Node>;
-    ghost var Repr: set<object>
-
-    function Read() : L.Node
-    requires box.Inv()
-    reads this, box, box.Repr
-    {
-      box.Read()
-    }
-
-    constructor(pivotTable: Pivots.PivotTable, children: Option<seq<BT.G.Reference>>, linear buckets: lseq<MutBucket>)
-    requires MutBucket.InvLseq(buckets)
-    ensures Inv()
-    ensures Read().pivotTable == pivotTable
-    ensures Read().children == children
-    ensures Read().buckets == buckets
-    ensures fresh(this.Repr)
-    {
-      linear var node := L.Node.Alloc(pivotTable, children, buckets);
-      box := new BoxedLinearOption(node, ToDestructor(L.FreeNode));
-      new;
-      Repr := {this} + box.Repr;
-    }
-
-    constructor InitFromNode(linear node: L.Node)
-    requires node.Inv()
-    ensures Inv()
-    ensures Read() == node
-    ensures fresh(this.Repr)
-    {
-      box := new BoxedLinearOption(node, ToDestructor(L.FreeNode));
-      new;
-      Repr := {this} + box.Repr;
-    }
-
-    function I() : (result: L.BT.G.Node)
-    reads this, this.box.Repr
-    requires Inv()
-    {
-      this.Read().I()
-    }
-
-    predicate Inv()
-    ensures Inv() ==> this in this.Repr
-    reads this, this.Repr
-    {
-      && this.box in this.Repr
-      && this.Repr == {this} + this.box.Repr
-      && this.box.Inv()
-      && this.box.Has()
-      && this.box.DataInv == L.FreeNode.requires
-      && this.Read().Inv()
-    }
-
-    method SplitParent(slot: uint64, pivot: Key, left_childref: L.BT.G.Reference, right_childref: L.BT.G.Reference)
-    requires Inv()
-    requires L.BT.WFNode(I())
-    requires Read().children.Some?
-    requires 0 <= slot as int < |Read().children.value|
-    requires 0 <= slot as int < |Read().buckets|
-    ensures Inv()
-    ensures I() == (L.BT.SplitParent(old(I()), pivot, slot as int, left_childref, right_childref))
-    ensures Repr == old(Repr)
-    modifies this.Repr
-    {
-      linear var n := this.box.Take();
-      inout n.SplitParent(slot, pivot, left_childref, right_childref);
-      this.box.Give(n);
-    }
-
-    method InsertKeyValue(key: Key, msg: Message)
-    requires Inv()
-    requires L.BT.WFNode(I())
-    requires L.Pivots.BoundedKey(Read().pivotTable, key)
-    requires WeightBucketList(MutBucket.ILseq(Read().buckets)) + WeightKey(key) + WeightMessage(msg) < 0x1_0000_0000_0000_0000
-    ensures Inv();
-    ensures I() == old(L.BT.NodeInsertKeyValue(I(), key, msg))
-    ensures Repr == old(Repr)
-    modifies this.Repr
-    {
-      linear var n := this.box.Take();
-      inout n.InsertKeyValue(key, msg);
-      this.box.Give(n);
-    }
-
-    method UpdateSlot(slot: uint64, linear bucket: MutBucket, childref: BT.G.Reference) 
-    requires Inv()
-    requires bucket.Inv()
-    requires Read().children.Some?
-    requires 0 <= slot as int < |Read().children.value|
-    requires 0 <= slot as int < |Read().buckets|
-    requires slot as int + 1 < 0x1_0000_0000_0000_0000
-    ensures Inv()
-    ensures I() == L.BT.G.Node(
-        old(I()).pivotTable,
-        Some(old(I()).children.value[slot as int := childref]),
-        old(I()).buckets[slot as int := bucket.bucket]
-      )
-    ensures Repr == old(Repr)
-    modifies this.Repr
-    {
-      linear var n := this.box.Take();  
-      inout n.UpdateSlot(slot, bucket, childref);
-      this.box.Give(n);
-    }
-
-    method BucketsWellMarshalled() returns (result: bool)
-    requires Inv()
-    requires |Read().buckets| < Uint64UpperBound()
-    ensures result == BucketsLib.BucketListWellMarshalled(MutBucket.ILseq(Read().buckets))
-    {
-      result := L.Node.BucketsWellMarshalled(this.box.Borrow());
-    }
-
-    method SplitChildLeft(num_children_left: uint64)
-    returns (node': Node)
-    requires Inv()
-    requires |Read().pivotTable| < Uint64UpperBound()
-    requires 0 <= num_children_left as int - 1 <= |Read().pivotTable| - 2
-    requires Read().children.Some? ==> 0 <= num_children_left as int <= |Read().children.value|
-    requires 0 <= num_children_left as int <= |Read().buckets|
-    ensures node'.Inv()
-    ensures node'.I() == L.BT.SplitChildLeft(I(), num_children_left as int)
-    ensures fresh(node'.Repr)
-    {
-      linear var lnode' := L.Node.SplitChildLeft(this.box.Borrow(), num_children_left);
-      node' := new Node.InitFromNode(lnode');
-    }
-
-    method SplitChildRight(num_children_left: uint64)
-    returns (node': Node)
-    requires Inv()
-    requires 0 <= num_children_left as int <= |Read().pivotTable| - 1
-    requires Read().children.Some? ==> 0 <= num_children_left as int <= |Read().children.value|
-    requires 0 <= num_children_left as int <= |Read().buckets|
-    ensures node'.Inv()
-    ensures node'.I() == L.BT.SplitChildRight(I(), num_children_left as int)
-    ensures fresh(node'.Repr)
-    {
-      linear var lnode' := L.Node.SplitChildRight(this.box.Borrow(), num_children_left);
-      node' := new Node.InitFromNode(lnode');
-    }
-
-    method CutoffNode(lbound: Key, rbound: Option<Key>)
-    returns (node' : Node)
-    requires Inv()
-    requires BT.WFNode(I())
-    requires BT.ValidSplitKey(I(), lbound, rbound)
-    ensures node'.Inv()
-    ensures node'.I() == L.BT.CutoffNode(I(), lbound, rbound)
-    ensures fresh(node'.Repr)
-    {
-      linear var lnode' := L.Node.CutoffNode(this.box.Borrow(), lbound, rbound);
-      node' := new Node.InitFromNode(lnode');
-    }
-
-    method GetBucketsLen() returns (len: uint64)
-    requires Inv()
-    ensures len as nat == |Read().buckets|
-    {
-      len := L.Node.GetBucketsLen(this.box.Borrow());
-    }
-
-    method GetChildren() returns (children: Option<seq<BT.G.Reference>>)
-    requires Inv()
-    ensures children == Read().children
-    {
-      children := L.Node.GetChildren(this.box.Borrow());
-    }
-
-    method GetPivots() returns (pivots: Pivots.PivotTable)
-    requires Inv()
-    ensures pivots == Read().pivotTable
-    {
-      pivots := L.Node.GetPivots(this.box.Borrow());
-    }
-
-    method BoundedBucket(pivots: Pivots.PivotTable, slot: uint64) returns (result: bool)
-    requires Inv()
-    requires |pivots| < 0x4000_0000_0000_0000
-    requires Pivots.WFPivots(pivots)
-    requires slot as nat < |Read().buckets|
-    ensures result == Pivots.BoundedKeySeq(pivots, Read().buckets[slot as nat].I().keys)
-    {
-      result := L.Node.BoundedBucket(this.box.Borrow(), pivots, slot);
-    }
   }
 }
