Impl/SplitImpl.i.dfy
@@ -5,8 +5,11 @@ module SplitImpl {
   import opened IOImpl
   import opened BookkeepingImpl
   import SplitModel
+  import SM = StateModel
+  import IM = IOModel
   import opened StateImpl
-  import opened BoxNodeImpl
+  import opened NodeImpl
+  import CacheImpl
   import opened DiskOpImpl
 
   import opened Options
@@ -24,141 +27,15 @@ module SplitImpl {
 
   import opened NativeTypes
 
-  method splitBookkeeping(s: ImplVariables, left_childref: BT.G.Reference, right_childref: BT.G.Reference, parentref: BT.G.Reference, fused_parent_children: seq<BT.G.Reference>, left_child: Node, right_child: Node, slot: uint64)
-  requires Inv(s)
-  requires 0 <= slot as int < |fused_parent_children|
-  requires slot as int < MaxNumChildren()
-  requires left_child.Inv()
-  requires right_child.Inv()
-  requires left_child.Repr !! s.Repr()
-  requires right_child.Repr !! s.Repr()
-  requires s.ready
-  requires BookkeepingModel.ChildrenConditions(s.I(), left_child.Read().children)
-  requires BookkeepingModel.ChildrenConditions(s.I(), right_child.Read().children)
-  requires BookkeepingModel.ChildrenConditions(s.I(), Some(fused_parent_children))
-  requires |fused_parent_children| < MaxNumChildren()
-  requires |s.ephemeralIndirectionTable.I().graph| <= IndirectionTableModel.MaxSize() - 3
-  modifies s.lru.Repr
-  modifies s.ephemeralIndirectionTable.Repr
-  modifies s.blockAllocator.Repr
-  ensures s.ready
-  ensures s.W()
-  ensures forall o | o in s.lru.Repr :: o in old(s.lru.Repr) || fresh(o)
-  ensures forall o | o in s.ephemeralIndirectionTable.Repr :: o in old(s.ephemeralIndirectionTable.Repr) || fresh(o)
-  ensures forall o | o in s.blockAllocator.Repr :: o in old(s.blockAllocator.Repr) || fresh(o)
-  ensures s.I() == SplitModel.splitBookkeeping(old(s.I()), left_childref, right_childref, parentref, fused_parent_children, left_child.I(), right_child.I(), slot as int);
+  method computeValidSplitKey(cache: CacheImpl.MutCache, ref: BT.G.Reference,
+    pivots: PivotTable, lpivot: Key, rpivot: Option<Key>)
+  returns (b: bool)
+  requires cache.Inv()
+  requires cache.ptr(ref).Some?
+  requires cache.I()[ref].pivotTable == pivots
+  requires BT.WFNode(cache.I()[ref])
+  ensures BT.ValidSplitKey(cache.I()[ref], lpivot, rpivot) == b
   {
-    SplitModel.reveal_splitBookkeeping();
-
-    BookkeepingModel.lemmaChildrenConditionsPreservedWriteBookkeeping(s.I(), left_childref, left_child.Read().children, right_child.Read().children);
-    BookkeepingModel.lemmaChildrenConditionsPreservedWriteBookkeeping(s.I(), left_childref, left_child.Read().children, Some(fused_parent_children));
-    BookkeepingModel.lemmaRefInGraphOfWriteBookkeeping(s.I(), left_childref, left_child.Read().children);
-
-    var leftchild_children := left_child.GetChildren();
-    writeBookkeeping(s, left_childref, leftchild_children);
-
-    BookkeepingModel.lemmaChildrenConditionsPreservedWriteBookkeeping(s.I(), right_childref, right_child.Read().children, Some(fused_parent_children));
-    BookkeepingModel.lemmaRefInGraphOfWriteBookkeeping(s.I(), right_childref, right_child.Read().children);
-    BookkeepingModel.lemmaRefInGraphPreservedWriteBookkeeping(s.I(), right_childref, right_child.Read().children, left_childref);
-
-    var rightchild_children := right_child.GetChildren();
-    writeBookkeeping(s, right_childref, rightchild_children);
-
-    BookkeepingModel.lemmaChildrenConditionsOfReplace1With2(s.I(), fused_parent_children, slot as int, left_childref, right_childref);
-
-    var rep := Replace1with2(fused_parent_children, left_childref, right_childref, slot);
-    writeBookkeeping(s, parentref, Some(rep));
-  }
-
-  method splitCacheChanges(s: ImplVariables, left_childref: BT.G.Reference,
-      right_childref: BT.G.Reference, parentref: BT.G.Reference, slot: uint64, num_children_left: uint64, pivot: Key, left_child: Node, right_child: Node)
-  requires s.ready
-  requires s.W()
-  requires s.cache.ptr(parentref).Some?
-  requires BT.WFNode(s.cache.ptr(parentref).value.I())
-  requires s.cache.ptr(parentref).value.I().children.Some?
-  requires 0 <= slot as int < |s.cache.ptr(parentref).value.I().children.value|
-  requires left_child.Inv()
-  requires right_child.Inv()
-  requires left_child.Repr !! s.Repr()
-  requires right_child.Repr !! s.Repr()
-  requires left_child.Repr !! right_child.Repr
-  requires |s.cache.I()| <= 0x10000 - 2
-  requires left_childref != parentref
-  requires right_childref != parentref
-  requires PivotInsertable(s.cache.I()[parentref].pivotTable, (slot+1) as int, pivot)
-
-  modifies s.Repr()
-  modifies left_child.Repr // not really but it's easier to include this
-  modifies right_child.Repr
-
-  ensures s.W()
-  ensures (forall o | o in s.Repr() :: o in old(s.Repr()) || o in old(left_child.Repr) || o in old(right_child.Repr) || fresh(o))
-  ensures s.I() == SplitModel.splitCacheChanges(old(s.I()), left_childref, right_childref, parentref, slot as int, num_children_left as int, pivot, old(left_child.I()), old(right_child.I()))
-  ensures s.ready
-  {
-    SplitModel.reveal_splitCacheChanges();
-    s.cache.Insert(left_childref, left_child);
-    s.cache.Insert(right_childref, right_child);
-    s.cache.SplitParent(parentref, slot as uint64, pivot, left_childref, right_childref);
-  }
-
-  method splitDoChanges(s: ImplVariables, child: Node,
-      left_childref: BT.G.Reference, right_childref: BT.G.Reference, parentref: BT.G.Reference,
-      fused_parent: Node, fused_parent_children: seq<BT.G.Reference>, slot: uint64)
-  requires Inv(s)
-  requires child.Inv()
-  requires fused_parent.Inv()
-  requires s.ready
-  requires parentref in s.cache.I()
-  requires s.cache.I()[parentref] == fused_parent.I()
-  requires BT.WFNode(fused_parent.I());
-  requires BT.WFNode(child.I());
-  requires s.cache.I()[parentref].children.Some?
-  requires 0 <= slot as int < |s.cache.I()[parentref].children.value|
-  requires 0 <= slot as int < |fused_parent_children|
-  requires left_childref != parentref
-  requires right_childref != parentref
-  requires |child.Read().buckets| >= 2
-  requires BookkeepingModel.ChildrenConditions(s.I(), Some(fused_parent_children))
-  requires BookkeepingModel.ChildrenConditions(s.I(), child.Read().children)
-  requires |fused_parent_children| < MaxNumChildren()
-  requires |s.ephemeralIndirectionTable.I().graph| <= IndirectionTableModel.MaxSize() - 3
-
-  modifies s.Repr()
-
-  ensures WellUpdated(s)
-  ensures s.I() == SplitModel.splitDoChanges(old(s.I()), old(child.I()), left_childref, right_childref, parentref, fused_parent_children, slot as int)
-  ensures s.ready
-  {
-    var len := child.GetBucketsLen();
-    var num_children_left := len / 2;
-    var pivots := child.GetPivots();
-    var pivot := ComputeGetKey(pivots, num_children_left);
-    
-    SplitModel.reveal_splitDoChanges();
-
-    var parent_pivots := fused_parent.GetPivots();
-    var insertable := ComputePivotInsertable(parent_pivots, slot+1, pivot);
-    if insertable {
-      SplitModel.lemmaChildrenConditionsSplitChild(s.I(), child.I(), num_children_left as int);
-
-      var left_child := child.SplitChildLeft(num_children_left);
-      var right_child := child.SplitChildRight(num_children_left);
-
-      splitBookkeeping(s, left_childref, right_childref, parentref, fused_parent_children, left_child, right_child, slot as uint64);
-      splitCacheChanges(s, left_childref, right_childref, parentref, slot as uint64, num_children_left as uint64, pivot, left_child, right_child);
-    } else {
-      print "giving up; split can't run because new pivots will not be strictly sorted";
-    }
-  }
-
-  method computeValidSplitKey(node: Node, lpivot: Key, rpivot: Option<Key>) returns (b: bool)
-  requires node.Inv()
-  requires BT.WFNode(node.I())
-  ensures BT.ValidSplitKey(node.I(), lpivot, rpivot) == b
-  {
-    var pivots := node.GetPivots();
     var len := |pivots| as uint64;
     var valid := ComputeBoundedKey(pivots, lpivot);
     if !valid {
@@ -188,19 +65,199 @@ module SplitImpl {
     return true;
   }
 
+  method splitBookkeeping(s: ImplVariables, left_childref: BT.G.Reference,
+    right_childref: BT.G.Reference, parentref: BT.G.Reference, 
+    fparent_children: seq<BT.G.Reference>, shared left_child: Node, 
+    shared right_child: Node, slot: uint64)
+  requires Inv(s)
+  requires 0 <= slot as int < |fparent_children|
+  requires slot as int < MaxNumChildren()
+  requires left_child.Inv()
+  requires right_child.Inv()
+  requires s.ready
+  requires BookkeepingModel.ChildrenConditions(s.I(), left_child.children)
+  requires BookkeepingModel.ChildrenConditions(s.I(), right_child.children)
+  requires BookkeepingModel.ChildrenConditions(s.I(), Some(fparent_children))
+  requires |fparent_children| < MaxNumChildren()
+  requires |s.ephemeralIndirectionTable.I().graph| <= IndirectionTableModel.MaxSize() - 3
+  modifies s.lru.Repr
+  modifies s.ephemeralIndirectionTable.Repr
+  modifies s.blockAllocator.Repr
+  ensures s.ready
+  ensures s.W()
+  ensures forall o | o in s.lru.Repr :: o in old(s.lru.Repr) || fresh(o)
+  ensures forall o | o in s.ephemeralIndirectionTable.Repr :: o in old(s.ephemeralIndirectionTable.Repr) || fresh(o)
+  ensures forall o | o in s.blockAllocator.Repr :: o in old(s.blockAllocator.Repr) || fresh(o)
+  ensures s.I() == SplitModel.splitBookkeeping(old(s.I()), left_childref, right_childref, 
+    parentref, fparent_children, left_child.I(), right_child.I(), slot as int)
+  {
+    SplitModel.reveal_splitBookkeeping();
+
+    BookkeepingModel.lemmaChildrenConditionsPreservedWriteBookkeeping(s.I(), left_childref, left_child.children, right_child.children);
+    BookkeepingModel.lemmaChildrenConditionsPreservedWriteBookkeeping(s.I(), left_childref, left_child.children, Some(fparent_children));
+    BookkeepingModel.lemmaRefInGraphOfWriteBookkeeping(s.I(), left_childref, left_child.children);
+
+    writeBookkeeping(s, left_childref, left_child.children);
+
+    BookkeepingModel.lemmaChildrenConditionsPreservedWriteBookkeeping(s.I(), right_childref, right_child.children, Some(fparent_children));
+    BookkeepingModel.lemmaRefInGraphOfWriteBookkeeping(s.I(), right_childref, right_child.children);
+    BookkeepingModel.lemmaRefInGraphPreservedWriteBookkeeping(s.I(), right_childref, right_child.children, left_childref);
+
+    writeBookkeeping(s, right_childref, right_child.children);
+
+    BookkeepingModel.lemmaChildrenConditionsOfReplace1With2(s.I(), fparent_children, slot as int, left_childref, right_childref);
+
+    var rep := Replace1with2(fparent_children, left_childref, right_childref, slot);
+    writeBookkeeping(s, parentref, Some(rep));
+  }
+
+  method splitCacheChanges(s: ImplVariables, left_childref: BT.G.Reference,
+      right_childref: BT.G.Reference, parentref: BT.G.Reference, slot: uint64, 
+      num_children_left: uint64, pivot: Key, linear left_child: Node, linear right_child: Node)
+  requires s.ready
+  requires s.W()
+  requires s.cache.ptr(parentref).Some?
+  requires BT.WFNode(s.cache.I()[parentref])
+  requires s.cache.ptr(parentref).value.I().children.Some?
+  requires 0 <= slot as int < |s.cache.ptr(parentref).value.I().children.value|
+  requires left_child.Inv()
+  requires right_child.Inv()
+  requires |s.cache.I()| <= 0x10000 - 2
+  requires left_childref != parentref
+  requires right_childref != parentref
+  requires PivotInsertable(s.cache.I()[parentref].pivotTable, (slot+1) as int, pivot)
+  modifies s.Repr()
+  ensures s.W()
+  ensures (forall o | o in s.Repr() :: o in old(s.Repr()) || fresh(o))
+  ensures s.I() == SplitModel.splitCacheChanges(old(s.I()), left_childref, right_childref,
+    parentref, slot as int, num_children_left as int, pivot, left_child.I(), right_child.I())
+  ensures s.ready
+  {
+    SplitModel.reveal_splitCacheChanges();
+    s.cache.Insert(left_childref, left_child);
+    s.cache.Insert(right_childref, right_child);
+    s.cache.SplitParent(parentref, slot as uint64, pivot, left_childref, right_childref);
+  }
+
+  method splitDoChanges(s: ImplVariables, linear child: Node, left_childref: BT.G.Reference,
+      right_childref: BT.G.Reference, parentref: BT.G.Reference, fparent_pivots: PivotTable,
+      fparent_children: seq<BT.G.Reference>, slot: uint64)
+  requires s.ready
+  requires Inv(s)
+  requires child.Inv()
+  requires BT.WFNode(child.I())
+  requires s.cache.ptr(parentref).Some?
+  requires BT.WFNode(s.cache.I()[parentref])
+  requires fparent_pivots == s.cache.I()[parentref].pivotTable
+  requires Some(fparent_children) == s.cache.I()[parentref].children
+  requires 0 <= slot as int < |fparent_children|
+  requires |fparent_children| < MaxNumChildren()
+  requires |child.buckets| >= 2
+  requires left_childref != parentref
+  requires right_childref != parentref
+  requires BookkeepingModel.ChildrenConditions(s.I(), Some(fparent_children))
+  requires BookkeepingModel.ChildrenConditions(s.I(), child.children)
+  requires |s.ephemeralIndirectionTable.I().graph| <= IndirectionTableModel.MaxSize() - 3
+  modifies s.Repr()
+  ensures WellUpdated(s)
+  ensures s.I() == SplitModel.splitDoChanges(old(s.I()), old(child.I()), left_childref,
+    right_childref, parentref, fparent_children, slot as int)
+  ensures s.ready
+  {
+    var len := lseq_length_as_uint64(child.buckets);
+    var num_children_left := len / 2;
+    var pivot := ComputeGetKey(child.pivotTable, num_children_left);
+    
+    SplitModel.reveal_splitDoChanges();
+
+    var insertable := ComputePivotInsertable(fparent_pivots, slot+1, pivot);
+    if insertable {
+      SplitModel.lemmaChildrenConditionsSplitChild(s.I(), child.I(), num_children_left as int);
+
+      linear var left_child := child.SplitChildLeft(num_children_left);
+      linear var right_child := child.SplitChildRight(num_children_left);
+
+      splitBookkeeping(s, left_childref, right_childref, parentref,
+        fparent_children, left_child, right_child, slot as uint64);
+      splitCacheChanges(s, left_childref, right_childref, parentref,
+        slot as uint64, num_children_left as uint64, pivot, left_child, right_child);
+    } else {
+      print "giving up; split can't run because new pivots will not be strictly sorted";
+    }
+    var _ := FreeNode(child);
+  }
+
+  method splitChild(s: ImplVariables, parentref: BT.G.Reference, 
+    childref: BT.G.Reference, slot: uint64, lbound: Key, ubound: Option<Key>,
+    fparent_pivots: PivotTable, fparent_children: Option<seq<BT.G.Reference>>)
+  requires s.ready
+  requires Inv(s)
+  requires s.cache.ptr(childref).Some?
+  requires s.cache.ptr(parentref).Some?
+  requires s.cache.I()[parentref].children.Some?
+  requires fparent_pivots == s.cache.I()[parentref].pivotTable
+  requires fparent_children == s.cache.I()[parentref].children
+  requires 0 <= slot as int < |fparent_children.value|
+  requires fparent_children.value[slot] == childref
+  requires |fparent_children.value| < MaxNumChildren()
+  requires BT.ValidSplitKey(s.cache.I()[childref], lbound, ubound)
+  requires BookkeepingModel.ChildrenConditions(s.I(), fparent_children)
+  requires BookkeepingModel.ChildrenConditions(s.I(), s.cache.I()[childref].children)
+  requires |s.ephemeralIndirectionTable.I().graph| <= IndirectionTableModel.MaxSize() - 3
+  modifies s.Repr()
+  ensures s.ready
+  ensures WellUpdated(s)
+  ensures s.I() == SplitModel.splitChild(old(s.I()), parentref, childref, slot as int, lbound, ubound)
+  {
+    SplitModel.reveal_splitChild();
+
+    linear var child := s.cache.NodeCutOff(childref, lbound, ubound);
+    assert child.I() == BT.CutoffNode(s.cache.I()[childref], lbound, ubound);
+    SplitModel.lemmaChildrenConditionsCutoffNode(s.I(), s.cache.I()[childref], lbound, ubound);
+    assert BT.WFNode(child.I());
+
+    if (|child.pivotTable| as uint64 == 2) {
+      // TODO there should be an operation which just
+      // cuts off the node and doesn't split it.
+      print "giving up; doSplit can't run because child pivots can't be splitted\n";
+      var _ := FreeNode(child);
+    } else {
+      var len := lseq_length_as_uint64(child.buckets);
+      var num_children_left := len / 2;
+      var pivot := ComputeGetKey(child.pivotTable, num_children_left);
+
+      BookkeepingModel.getFreeRefDoesntEqual(s.I(), parentref);
+
+      var left_childref := getFreeRef(s);
+      if left_childref.None? {
+        print "giving up; doSplit can't allocate left_childref\n";
+        var _ := FreeNode(child);
+      } else {
+        BookkeepingModel.getFreeRef2DoesntEqual(s.I(), left_childref.value, parentref);
+        var right_childref := getFreeRef2(s, left_childref.value);
+        if right_childref.None? {
+          print "giving up; doSplit can't allocate right_childref\n";
+          var _ := FreeNode(child);
+        } else {
+          splitDoChanges(s, child, left_childref.value, right_childref.value,
+            parentref, fparent_pivots, fparent_children.value, slot as uint64);
+        }
+      }
+    }
+  }
+
   method doSplit(s: ImplVariables, parentref: BT.G.Reference, childref: BT.G.Reference, slot: uint64)
   requires s.ready
   requires Inv(s)
-  requires childref in s.ephemeralIndirectionTable.I().graph
-  requires parentref in s.ephemeralIndirectionTable.I().graph
   requires s.cache.ptr(childref).Some?
   requires s.cache.ptr(parentref).Some?
+  requires childref in s.ephemeralIndirectionTable.I().graph
+  requires parentref in s.ephemeralIndirectionTable.I().graph
   requires s.cache.I()[parentref].children.Some?
   requires 0 <= slot as int < |s.cache.I()[parentref].children.value|
   requires s.cache.I()[parentref].children.value[slot] == childref
   requires |s.cache.I()[parentref].buckets| <= MaxNumChildren() - 1
   requires |s.ephemeralIndirectionTable.I().graph| <= IndirectionTableModel.MaxSize() - 3
-
   modifies s.Repr()
   ensures WellUpdated(s)
   ensures s.ready
@@ -216,16 +273,14 @@ module SplitImpl {
       }
     }
 
-    var fused_parent_opt := s.cache.GetOpt(parentref);
-    var fused_parent := fused_parent_opt.value;
-    var fused_child_opt := s.cache.GetOpt(childref);
-    var fused_child := fused_child_opt.value;
-
-    var fparent_pivots := fused_parent.GetPivots();
-    var fchild_pivots := fused_child.GetPivots();
+    ghost var fused_parent := s.cache.I()[parentref];
+    ghost var fused_child := s.cache.I()[childref]; 
+    var fparent_pivots, fparent_children := s.cache.GetNodeInfo(parentref);
+    var fchild_pivots, _ := s.cache.GetNodeInfo(childref);
 
     var childlbound := KeyspaceImpl.cmp(fchild_pivots[0], fparent_pivots[slot]);
-    var childubound := KeyspaceImpl.cmp(fparent_pivots[slot+1], fchild_pivots[|fchild_pivots| as uint64 -1]);
+    var childubound := KeyspaceImpl.cmp(fparent_pivots[slot+1], 
+      fchild_pivots[|fchild_pivots| as uint64 -1]);
 
     if childlbound > 0 || childubound > 0 {
       print "giving up; split can't run because splitted keys are not in bound";
@@ -241,51 +296,17 @@ module SplitImpl {
       var ukey := ComputeGetKey(fparent_pivots, slot+1);
       ubound := Some(ukey);
     }
-    assert lbound == BT.getlbound(fused_parent.I(), slot as int);
-    assert ubound == BT.getubound(fused_parent.I(), slot as int);
+    assert lbound == BT.getlbound(fused_parent, slot as int);
+    assert ubound == BT.getubound(fused_parent, slot as int);
 
-    var childvalid := computeValidSplitKey(fused_child, lbound, ubound);
-    var parentvalid := computeValidSplitKey(fused_parent, lbound, ubound);
+    var childvalid := computeValidSplitKey(s.cache, childref, fchild_pivots, lbound, ubound);
+    var parentvalid := computeValidSplitKey(s.cache, parentref, fparent_pivots, lbound, ubound);
 
     if childvalid && parentvalid {
-      assert BT.ValidSplitKey(fused_parent.I(), lbound, ubound);
-      assert BT.ValidSplitKey(fused_child.I(), lbound, ubound);
-      SplitModel.lemmaChildrenConditionsCutoffNode(s.I(), fused_child.I(), lbound, ubound);
-    
-      var child := fused_child.CutoffNode(lbound, ubound);
-      assert BT.WFNode(child.I());
-
-      var child_pivots := child.GetPivots();
-      if (|child_pivots| as uint64 == 2) {
-        // TODO there should be an operation which just
-        // cuts off the node and doesn't split it.
-        print "giving up; doSplit can't run because child pivots can't be splitted\n";
-        return;
-      }
-
-      var len := child.GetBucketsLen();
-      var num_children_left := len / 2;
-      var pivot := ComputeGetKey(child_pivots, num_children_left);
-
-      BookkeepingModel.getFreeRefDoesntEqual(s.I(), parentref);
-
-      var left_childref := getFreeRef(s);
-      if left_childref.None? {
-        print "giving up; doSplit can't allocate left_childref\n";
-        return;
-      }
-
-      BookkeepingModel.getFreeRef2DoesntEqual(s.I(), left_childref.value, parentref);
-
-      var right_childref := getFreeRef2(s, left_childref.value);
-      if right_childref.None? {
-        print "giving up; doSplit can't allocate right_childref\n";
-        return;
-      }
-
-      var fparent_children := fused_parent.GetChildren();
-      splitDoChanges(s, child, left_childref.value, right_childref.value,
-        parentref, fused_parent, fparent_children.value, slot as uint64);
+      assert BT.ValidSplitKey(fused_parent, lbound, ubound);
+      assert BT.ValidSplitKey(fused_child, lbound, ubound);
+     
+      splitChild(s, parentref, childref, slot, lbound, ubound, fparent_pivots, fparent_children);
     } else {
       print "giving up; split can't run because bounds checking failed";
     }
