Impl/InsertImpl.i.dfy
@@ -1,7 +1,7 @@
 include "IOImpl.i.dfy"
 include "BookkeepingImpl.i.dfy"
 include "InsertModel.i.dfy"
-include "FlushPolicyImpl.i.dfy"
+// include "FlushPolicyImpl.i.dfy"
 include "MainDiskIOHandler.s.dfy"
 include "../lib/Base/Option.s.dfy"
 include "../lib/Base/Sets.i.dfy"
@@ -14,7 +14,7 @@ module InsertImpl {
   import opened BookkeepingImpl
   import opened InsertModel
   import opened StateImpl
-  import opened FlushPolicyImpl
+  // import opened FlushPolicyImpl
   import opened BucketImpl
   import opened DiskOpImpl
   import opened MainDiskIOHandler
@@ -32,7 +32,7 @@ module InsertImpl {
   import opened BucketWeights
   import opened Bounds
 
-  import opened BoxNodeImpl
+  import opened NodeImpl
   import opened BoundedPivotsLib
 
   method InsertKeyValue(s: ImplVariables, key: Key, value: Value)
@@ -86,8 +86,8 @@ module InsertImpl {
       return;
     }
 
-    var rootLookup := s.cache.GetOpt(BT.G.Root());
-    if (rootLookup.None?) {
+    var rootLookup := s.cache.InCache(BT.G.Root());
+    if !rootLookup {
       if TotalCacheSize(s) <= MaxCacheSizeUint64() - 1 {
         PageInNodeReq(s, io, BT.G.Root());
         success := false;
@@ -97,8 +97,8 @@ module InsertImpl {
       }
       return;
     }
-
-    var pivots := rootLookup.value.GetPivots();
+ 
+    var pivots, _ := s.cache.GetNodeInfo(BT.G.Root());
     var bounded := ComputeBoundedKey(pivots, key);
     if !bounded {
       success := false;
@@ -106,12 +106,13 @@ module InsertImpl {
       return;
     }
 
-    var weightSeq := MutBucket.computeWeightOfSeq(rootLookup.value.box.Borrow().buckets);
+    var weightSeq := s.cache.NodeBucketsWeight(BT.G.Root());
     if WeightKeyUint64(key) + WeightMessageUint64(ValueMessage.Define(value)) + weightSeq
         <= MaxTotalBucketWeightUint64() {
       success := InsertKeyValue(s, key, value);
     } else {
-      runFlushPolicy(s, io);
+      assume false;
+      // runFlushPolicy(s, io);
       success := false;
     }
   }
