lib/DataStructures/LinearContentMutableMap.i.dfy
@@ -1,0 +1,1283 @@
+include "../Lang/LinearSequence.s.dfy"
+include "../Lang/LinearSequence.i.dfy"
+include "../Base/LinearOption.i.dfy"
+include "../Lang/Inout.i.dfy"
+
+include "../Lang/NativeTypes.s.dfy"
+include "../Base/Option.s.dfy"
+include "../Base/sequences.i.dfy"
+include "../Base/Sets.i.dfy"
+include "../Base/Maps.i.dfy"
+include "LinearMutableMapBase.i.dfy"
+
+//
+// Immutable (functional) model to support MutableMapImpl.  API provides an
+// iterator interface with a deterministic order for parsing/marshaling.
+// (That's why the API is/ more than just a Dafny map.)
+//
+// TODO(jonh): Here and elsewhere, Model files seem to be both
+// API (because callers use some of the definitions as 'public' ways
+// to reason about the behavior of the modeled Impl) and internal
+// proof (the logic half of the behavior of the Impl). It would be
+// nice to cleanly separate these concerns.
+//
+
+module LinearContentMutableMap {
+  import opened NativeTypes
+  import opened Options
+  import opened LinearOption
+  import opened Sequences
+  import opened Sets
+  import opened Maps
+
+  import opened LinearSequence_i
+  import opened LinearSequence_s
+  import opened Inout
+  import opened Base = LinearMutableMapBase
+
+  linear datatype lItem<V> = Empty | Entry(key: uint64, linear value: V) | Tombstone(key: uint64)
+  {
+    linear method FreeNonEntry()
+    requires !this.Entry? 
+    {
+      linear match this {
+        case Empty() => 
+        case Tombstone(key) =>
+      }
+    }
+
+    function toItem(): Item<V>
+    {
+      match this {
+        case Empty() => Base.Empty()
+        case Entry(key, value) => Base.Entry(key, value)
+        case Tombstone(key) => Base.Tombstone(key)
+      }
+    }
+  }
+
+  function toItems<V>(litems: lseq<lItem<V>>): (items: seq<Item<V>>)
+  ensures |items| == |litems|
+  {
+    var elements := lseqs(litems);
+    seq (|elements|, i requires 0 <= i < |elements| => elements[i].toItem())
+  }
+
+  linear datatype FixedSizeLinearHashMap<V> = FixedSizeLinearHashMap(
+    linear storage: lseq<lItem<V>>,
+    count: uint64,
+    ghost contents: map<uint64, Option<V>>)
+
+  function method Uint64SlotForKey<V>(shared self: FixedSizeLinearHashMap<V>, key: uint64): (result: uint64)
+  requires 0 < |self.storage| < 0x1_0000_0000_0000_0000
+  ensures ValidSlot(|self.storage|, Slot(result as nat))
+  ensures Slot(result as nat) == SlotForKey(|self.storage|, key)
+  {
+    var h := hash64(key);
+    var storageLength := lseq_length_as_uint64(self.storage);
+    h % (storageLength as uint64)
+  }
+
+  predicate FixedSizeInv<V>(self: FixedSizeLinearHashMap<V>)
+  {
+    && 128 <= |self.storage| < 0x1_0000_0000_0000_0000
+    && (self.count as nat) < 0x1_0000_0000_0000_0000
+    && self.count as nat < |self.storage|
+
+    && |self.contents| == (self.count as nat)
+    && lseq_has_all(self.storage)
+    && SeqMatchesContentKeys(toItems(self.storage), self.contents)
+    && EntriesMatchContentValue(toItems(self.storage), self.contents)
+    && TombstonesMatchContentValue(toItems(self.storage), self.contents)
+  }
+
+  predicate IsConstructorFromSize<V>(size: nat, self: FixedSizeLinearHashMap<V>)  
+  {
+    && |self.storage| == size
+    && self.count == 0
+    && self.contents == map[]
+    && (forall slot :: ValidSlot(|self.storage|, slot) ==> SlotIsEmpty(toItems(self.storage), slot))
+    && FixedSizeInv(self)
+  }
+
+  method ConstructorFromSize<V>(size: uint64) returns (linear self: FixedSizeLinearHashMap<V>)
+  requires 128 <= size
+  ensures IsConstructorFromSize(size as nat, self)
+  {
+    linear var storage := lseq_alloc(size);
+
+    var i := 0 as uint64;
+    while i < size
+      invariant i <= size
+      invariant size as nat == |storage|
+      invariant forall j | 0 <= j < i as nat :: lseq_has(storage)[j]
+      invariant forall j | i as nat <= j < size as nat :: !lseq_has(storage)[j]
+      invariant forall slot :: ValidSlot(|storage|, slot) && 0 <= slot.slot < i as nat 
+          ==> SlotIsEmpty(toItems(storage), slot)
+    {
+      linear var item := lItem.Empty();
+      lseq_give_inout(inout storage, i, item);
+      i := i + 1;
+    }
+
+    self := FixedSizeLinearHashMap(
+     /* storage := */ storage,
+     /* count := */ 0,
+     /* contents := */ map[]);
+  }
+
+  lemma allNonEmptyImpliesCountEqStorageSize<V>(self: FixedSizeLinearHashMap<V>)
+  requires FixedSizeInv(self)
+  ensures (forall j | 0 <= j < |self.storage| :: !self.storage[j].Empty?)
+      ==> self.count as int == |self.storage|
+  {
+    var elements := self.storage;
+    if forall j | 0 <= j < |elements| :: !elements[j].Empty? {
+      var elementIndices := set i | 0 <= i < |elements|;
+      assert IndexSetThrough(toItems(elements), |elements|) == elementIndices; // trigger
+      CardinalityOfSetsOfSequenceIndices(toItems(elements), elementIndices);
+      IndexSetMatchesContents(toItems(elements), self.contents);
+    }
+  }
+
+  function {:opaque} getEmptyWitness<V>(self: FixedSizeLinearHashMap<V>, i: uint64) : (res : uint64)
+  requires FixedSizeInv(self)
+  requires 0 <= i as int <= |self.storage|
+  requires forall j | 0 <= j < i as int :: !self.storage[j].Empty?
+  requires self.count as int < |self.storage|
+  decreases |self.storage| - i as int
+  ensures 0 <= res as int < |self.storage|
+  ensures self.storage[res as int].Empty?
+  {
+    allNonEmptyImpliesCountEqStorageSize(self);
+
+    if self.storage[i as int].Empty? then
+      i
+    else
+      getEmptyWitness(self, i+1)
+  }
+
+  function method ProbeIterate<V>(shared self: FixedSizeLinearHashMap<V>, key: uint64, slotIdx: uint64)
+      : (foundSlotIdx: uint64)
+  requires FixedSizeInv(self)
+  requires 0 <= slotIdx as int < |self.storage|
+
+  // We use the emptyWitness to prove termination.
+  // We will necessarily terminate when we reach this index,
+  // if not earlier.
+  decreases var wit := getEmptyWitness(self, 0);
+    if slotIdx > wit
+      then wit as int - slotIdx as int + |self.storage|
+      else wit as int - slotIdx as int
+
+  ensures 0 <= foundSlotIdx as int < |self.storage|
+  {
+    shared var item := lseq_peek(self.storage, slotIdx);
+    if item.Empty? || item.key == key then
+      slotIdx
+    else (
+      ProbeIterate(self, key, Uint64SlotSuccessorUint64(lseq_length_as_uint64(self.storage), slotIdx))
+    )
+  }
+
+  function method {:opaque} Probe<V>(shared self: FixedSizeLinearHashMap<V>, key: uint64): (foundSlotIdx: uint64)
+  requires FixedSizeInv(self)
+  requires self.count as int < |self.storage|
+  ensures 0 <= foundSlotIdx as int < |self.storage|
+  {
+    ProbeIterate(self, key, Uint64SlotForKey(self, key))
+  }
+
+  datatype ProbeResult<V> = ProbeResult(
+      slotIdx: uint64,
+      ghost startSlotIdx: uint64,
+      ghost ghostSkips: uint64)
+
+  lemma LemmaProbeResult<V>(self: FixedSizeLinearHashMap<V>, key: uint64)
+  returns (result : ProbeResult<V>)
+  requires FixedSizeInv(self)
+  ensures result.slotIdx == Probe(self, key)
+  ensures ValidSlot(|self.storage|, Slot(result.slotIdx as nat))
+  ensures ValidSlot(|self.storage|, Slot(result.startSlotIdx as nat))
+  ensures Slot(result.startSlotIdx as nat) == SlotForKey(|self.storage|, key)
+  ensures 0 <= result.ghostSkips
+  ensures result.slotIdx as nat == KthSlotSuccessor(|self.storage|, Slot(result.startSlotIdx as nat), result.ghostSkips as nat).slot
+  ensures key in self.contents ==> SlotExplainsKey(toItems(self.storage), result.ghostSkips as nat, key)
+  ensures key !in self.contents ==> FilledWithOtherKeys(toItems(self.storage), Slot(result.startSlotIdx as nat), result.ghostSkips as nat, key) 
+    && (self.storage[result.slotIdx as nat].Empty? || (self.storage[result.slotIdx as nat].Tombstone? && self.storage[result.slotIdx as nat].key == key))
+  ensures self.storage[result.slotIdx as nat].Entry? ==> key in self.contents && key == self.storage[result.slotIdx as nat].key
+  ensures self.storage[result.slotIdx as nat].Empty? ==> key !in self.contents
+  {
+    reveal_Probe();
+
+    var slotIdx := Uint64SlotForKey(self, key);
+    var startSlotIdx := slotIdx;
+    ghost var startSlot := Slot(startSlotIdx as nat);
+
+    ghost var viewFromStartSlot := View(toItems(self.storage), startSlotIdx as nat);
+    ViewsHaveConsistentCounts(toItems(self.storage), viewFromStartSlot, startSlotIdx as nat);
+    CountFilledMatchesIndexSet(toItems(self.storage));
+    IndexSetMatchesContents(toItems(self.storage), self.contents);
+
+    forall dist: nat | dist < |self.storage|
+    ensures viewFromStartSlot[dist] ==
+      self.storage[KthSlotSuccessor(|self.storage|, startSlot, dist).slot].toItem()
+    {
+      KthSlotSuccessorWrapsAround(|self.storage|, startSlot, dist); // observe
+    }
+
+    var skips := 0;
+    while true
+      invariant skips < (|self.storage| as uint64)
+      invariant slotIdx < (|self.storage| as uint64)
+      invariant |self.storage| == |viewFromStartSlot|
+      invariant toItems(self.storage)[startSlotIdx..] 
+        + toItems(self.storage)[..startSlotIdx] == viewFromStartSlot
+      invariant slotIdx as nat ==
+        KthSlotSuccessor(|self.storage|, startSlot, skips as nat).slot
+      invariant skips < (|self.storage| as uint64) ==> 
+        toItems(self.storage)[slotIdx] == viewFromStartSlot[skips]
+      invariant ValidSlot(|self.storage|, KthSlotSuccessor(|self.storage|, startSlot, skips as nat))
+      invariant FilledWithOtherKeys(toItems(self.storage), startSlot, skips as nat, key)
+      invariant CountFilled(viewFromStartSlot[..skips]) == skips as nat
+
+      invariant Probe(self, key) == ProbeIterate(self, key, slotIdx)
+
+      decreases var wit := getEmptyWitness(self, 0);
+        if slotIdx > wit
+          then wit as int - slotIdx as int + |self.storage|
+          else wit as int - slotIdx as int
+    {
+      if self.storage[slotIdx as nat].Empty? 
+        || (self.storage[slotIdx as nat].Tombstone? 
+        && self.storage[slotIdx as nat].key == key) {
+        result := ProbeResult(slotIdx, startSlotIdx, skips);
+        return;
+      } else if self.storage[slotIdx as nat].key == key {
+        assert EntryInSlotMatchesContents(toItems(self.storage), Slot(slotIdx as nat), self.contents); // observe
+        result := ProbeResult(slotIdx, startSlotIdx, skips);
+        return;
+      }
+
+      ghost var skipsBefore := skips;
+
+      // -- increment --
+      slotIdx := Uint64SlotSuccessor(|self.storage|, slotIdx);
+      skips := skips + 1;
+      // ---------------
+
+      assert viewFromStartSlot[..skips] == viewFromStartSlot[..skipsBefore] + [viewFromStartSlot[skipsBefore]]; // observe
+      CountFilledAdditive(viewFromStartSlot[..skipsBefore], [viewFromStartSlot[skipsBefore]]);
+
+      assert Probe(self, key) == ProbeIterate(self, key, slotIdx);
+
+      if skips == |self.storage| as uint64 {
+        forall ensures false
+        {
+          calc {
+            |self.storage|;
+            skips as nat;
+            CountFilled(viewFromStartSlot[..skips]);
+              { assert viewFromStartSlot[..skips] == viewFromStartSlot; } // observe
+            CountFilled(viewFromStartSlot);
+            |self.contents|;
+            self.count as nat;
+            < |self.storage|;
+          }
+        }
+      }
+    }
+  }
+  
+  predicate {:opaque} IsFixedSizeInsert<V> (self: FixedSizeLinearHashMap, key: uint64, value: V, 
+    self': FixedSizeLinearHashMap, replaced: lOption<V>)
+  requires FixedSizeInv(self)
+  requires self.count as nat < |self.storage| - 1
+  {
+    && var slotIdx := Probe(self, key);
+    && self'.contents == self.contents[key := Some(value)]
+    && toItems(self'.storage) == toItems(self.storage)[slotIdx as nat := Base.Entry(key, value)]
+    && match self.storage[slotIdx as nat] {
+        case Empty => (
+          && replaced == lNone
+          && self'.count == self.count + 1
+        )
+        case Tombstone(_) => (
+          && replaced == lNone
+          && self'.count == self.count
+        )
+        case Entry(_, value) => (
+          && replaced == lSome(value)
+          && self'.count == self.count
+        )
+      }
+    && lseq_has_all(self'.storage)
+  }
+
+  method FixedSizeInsert<V>(linear inout self: FixedSizeLinearHashMap, key: uint64, linear value: V)
+  returns (linear replaced: lOption<V>)
+  requires FixedSizeInv(old_self)
+  requires old_self.count as nat < |old_self.storage| - 1
+  ensures FixedSizeInv(self)
+  ensures self.contents == old_self.contents[key := Some(value)]
+  ensures key !in old_self.contents ==> replaced.lNone?
+  ensures key in old_self.contents ==> replaced.Option() == old_self.contents[key]
+  ensures replaced.lSome? ==> key in old_self.contents
+  ensures |self.storage| == |old_self.storage|
+  {
+    linear var entry := lItem.Entry(key, value);
+    replaced := FixedSizeInsertEntry(inout self, entry);
+  }
+
+  method FixedSizeInsertEntry<V>(linear inout self: FixedSizeLinearHashMap, linear entry: lItem<V>)
+  returns (linear replaced: lOption<V>)
+  requires entry.Entry?
+  requires FixedSizeInv(old_self)
+  requires old_self.count as nat < |old_self.storage| - 1
+  ensures FixedSizeInv(self)
+  ensures self.contents == old_self.contents[entry.key := Some(entry.value)]
+  ensures entry.key !in old_self.contents ==> replaced.lNone?
+  ensures entry.key in old_self.contents ==> replaced.Option() == old_self.contents[entry.key]
+  ensures replaced.lSome? ==> entry.key in old_self.contents
+  ensures |self.storage| == |old_self.storage|
+  {
+    reveal_IsFixedSizeInsert();
+    var slotIdx := Probe(self, entry.key);
+
+    ghost var contents := old_self.contents[entry.key := Some(entry.value)];
+    inout ghost self.contents := contents;
+    
+    linear var olditem := lseq_take_inout(inout self.storage, slotIdx);
+    lseq_give_inout(inout self.storage, slotIdx, entry);
+
+    if olditem.Empty? {
+      olditem.FreeNonEntry();
+      inout self.count := self.count + 1;
+      replaced := lNone;
+   } else if olditem.Tombstone? {
+      olditem.FreeNonEntry();
+      replaced := lNone;
+    } else {
+      linear var Entry(_, value) := olditem;
+      replaced := lSome(value);
+    }
+    LemmaFixedSizeInsert(old_self, entry.key, entry.value, self, replaced);
+  }
+
+  lemma LemmaFixedSizeInsert<V>(self: FixedSizeLinearHashMap, key: uint64, value: V, 
+    self': FixedSizeLinearHashMap, replaced: lOption<V>)
+  requires IsFixedSizeInsert.requires(self, key, value, self', replaced)
+  requires IsFixedSizeInsert(self, key, value, self', replaced)
+  ensures FixedSizeInv(self')
+  ensures self'.contents == self.contents[key := Some(value)]
+  ensures key !in self.contents ==> replaced.lNone?
+  ensures key in self.contents ==> replaced.Option() == self.contents[key]
+  ensures replaced.lSome? ==> key in self.contents
+  ensures |self'.storage| == |self.storage|
+  {
+    reveal_IsFixedSizeInsert();
+
+    var probeRes := LemmaProbeResult(self, key);
+    var slotIdx := probeRes.slotIdx;
+    var probeStartSlotIdx := probeRes.startSlotIdx;
+    var probeSkips := probeRes.ghostSkips;
+
+    forall explainedKey | explainedKey in self'.contents
+    ensures exists skips :: SlotExplainsKey(toItems(self'.storage), skips, explainedKey)
+    {
+      if key == explainedKey {
+        assert SlotExplainsKey(toItems(self'.storage), probeSkips as nat, key); // observe
+      } else {
+        var oldSkips :| SlotExplainsKey(toItems(self.storage), oldSkips, explainedKey);
+        assert SlotExplainsKey(toItems(self'.storage), oldSkips, explainedKey); // observe
+      }
+    }
+  
+    forall slot | ValidSlot(|self'.storage|, slot) && toItems(self'.storage)[slot.slot].Entry?
+    ensures && var item := toItems(self'.storage)[slot.slot];
+            && self'.contents[item.key] == Some(item.value)
+    {
+      var item := toItems(self'.storage)[slot.slot];
+      if slot != Slot(slotIdx as nat) {
+        if item.key == key {
+          assert TwoNonEmptyValidSlotsWithSameKey(toItems(self'.storage), slot, Slot(slotIdx as nat)); // observe
+          assert SameSlot(|self'.storage|, slot, Slot(slotIdx as nat)); // observe
+          assert false;
+        }
+      }
+    }
+    forall slot | ValidSlot(|self'.storage|, slot) && toItems(self'.storage)[slot.slot].Tombstone?
+    ensures && var item := self'.storage[slot.slot];
+            && self'.contents[item.key].None?
+    {
+      var item := self'.storage[slot.slot];
+      if slot != Slot(slotIdx as nat) {
+        if item.key == key {
+          assert TwoNonEmptyValidSlotsWithSameKey(toItems(self'.storage), slot, Slot(slotIdx as nat)); // observe
+          assert SameSlot(|self'.storage|, slot, Slot(slotIdx as nat)); // observe
+          assert false;
+        }
+      }
+    }
+  }
+
+  predicate IsFixedSizeUpdateBySlot<V>(self: FixedSizeLinearHashMap<V>, slotIdx: uint64, value: V,
+    self': FixedSizeLinearHashMap<V>, replaced: V)
+  requires FixedSizeInv(self)
+  requires 0 <= slotIdx as int < |self.storage|
+  requires self.storage[slotIdx as nat].Entry?
+  {
+    && var key := self.storage[slotIdx as nat].key;
+    && self'.count == self.count
+    && |self'.contents| == |self.contents|
+    && self'.contents == self.contents[key := Some(value)]
+    && replaced == self.storage[slotIdx as nat].value
+    && lseq_has_all(self'.storage)
+    && toItems(self'.storage) == toItems(self.storage)[slotIdx as nat := Base.Entry(key, value)]
+  }
+
+  method FixedSizeUpdateBySlot<V>(linear inout self: FixedSizeLinearHashMap<V>, slotIdx: uint64, linear value: V)
+  returns (linear replaced: V)
+  requires FixedSizeInv(old_self)
+  requires 0 <= slotIdx as int < |old_self.storage|
+  requires old_self.storage[slotIdx as nat].Entry?
+  ensures IsFixedSizeUpdateBySlot(old_self, slotIdx, value, self, replaced)
+  ensures FixedSizeInv(self)
+  {
+    linear var entry: lItem<V> := lseq_take_inout(inout self.storage, slotIdx);
+    linear var Entry(key, oldvalue) := entry;
+    lseq_give_inout(inout self.storage, slotIdx, lItem.Entry(key, value));
+    replaced := oldvalue;
+
+    inout ghost self.contents := self.contents[key := Some(value)];
+    assert EntryInSlotMatchesContents(toItems(old_self.storage), Slot(slotIdx as int), old_self.contents);
+    LemmaFixedSizeUpdateBySlot(old_self, slotIdx, value, self, replaced);
+  }
+
+  lemma LemmaFixedSizeUpdateBySlot<V>(self: FixedSizeLinearHashMap<V>, slotIdx: uint64, value: V,
+    self': FixedSizeLinearHashMap<V>, replaced: V)
+  requires IsFixedSizeUpdateBySlot.requires(self, slotIdx, value, self', replaced)
+  requires IsFixedSizeUpdateBySlot(self, slotIdx, value, self', replaced)
+  ensures FixedSizeInv(self')
+  {
+    var key := self.storage[slotIdx as nat].key;
+
+    forall explainedKey | explainedKey in self'.contents
+    ensures exists skips :: SlotExplainsKey(toItems(self'.storage), skips, explainedKey)
+    {
+      var oldSkips :| SlotExplainsKey(toItems(self.storage), oldSkips, explainedKey);
+      assert SlotExplainsKey(toItems(self'.storage), oldSkips, explainedKey); // observe
+    }
+  
+    forall slot | ValidSlot(|self'.storage|, slot)
+        && SlotIsEntry(toItems(self'.storage), slot)
+    ensures EntryInSlotMatchesContents(toItems(self'.storage), slot, self'.contents)
+    {
+      assert EntryInSlotMatchesContents(toItems(self.storage), slot, self.contents);
+      if self.storage[slot.slot].key == key {
+        assert TwoNonEmptyValidSlotsWithSameKey(toItems(self.storage), slot, Slot(slotIdx as int));
+      }
+    }
+
+    forall slot | ValidSlot(|self'.storage|, slot)
+        && toItems(self'.storage)[slot.slot].Tombstone?
+    ensures TombstoneInSlotMatchesContents(toItems(self'.storage), slot, self'.contents)
+    {
+      if slot.slot != slotIdx as nat && self.storage[slot.slot].key == key {
+        assert TwoNonEmptyValidSlotsWithSameKey(toItems(self'.storage), slot, Slot(slotIdx as nat)); // observe
+        assert SameSlot(|self'.storage|, slot, Slot(slotIdx as nat)); // observe
+        assert false;
+      }
+    }
+  }
+
+  function method IsEntry<V>(shared self: FixedSizeLinearHashMap<V>, key: uint64) : (b: bool)
+  requires FixedSizeInv(self)
+  ensures b == (key in self.contents && self.contents[key].Some?)
+  {
+    var slotIdx := Probe(self, key);
+    var b := lseq_peek(self.storage, slotIdx).Entry?;
+    assert b == (key in self.contents && self.contents[key].Some?) by {
+      var _ := LemmaProbeResult(self, key);
+    }
+    b
+  }
+
+  function method {:opaque} FixedSizeGet<V>(shared self: FixedSizeLinearHashMap<V>, key: uint64)
+    : (shared found: V)
+  requires FixedSizeInv(self)
+  requires IsEntry(self, key)
+  ensures key in self.contents && self.contents[key].Some?
+  {
+    var slotIdx := Probe(self, key);
+    lseq_peek(self.storage, slotIdx).value
+    // TODO(Jialin): update to return shared lOption<V>
+  }
+
+  lemma LemmaFixedSizeGet<V>(self: FixedSizeLinearHashMap<V>, key: uint64)
+  requires FixedSizeGet.requires(self, key)
+  requires key in self.contents && self.contents[key].Some?
+  ensures FixedSizeGet(self, key) == self.contents[key].value
+  {
+    reveal_FixedSizeGet();
+    var _ := LemmaProbeResult(self, key);
+  }
+
+  predicate IsFixedSizeRemove<V>(self: FixedSizeLinearHashMap<V>, key: uint64, 
+    self': FixedSizeLinearHashMap<V>, removed: lOption<V>)
+  requires FixedSizeInv(self)
+  {
+    && var slotIdx := Probe(self, key);
+    && (!self.storage[slotIdx as nat].Entry? ==> self' == self && removed == lNone)
+    && (self.storage[slotIdx as nat].Entry? ==> 
+      && self'.count == self.count
+      && self'.contents == self.contents[key := None]
+      && |self'.contents| == |self.contents|
+      && lseq_has_all(self'.storage)
+      && toItems(self'.storage) == toItems(self.storage)[slotIdx as nat := Base.Tombstone(key)]
+      && removed == lSome(self.storage[slotIdx as nat].value)
+    )
+    && (removed.lSome? <==> (key in self.contents && self.contents[key].Some?)) // leave this here for now
+  }
+  
+  method FixedSizeRemove<V>(linear inout self: FixedSizeLinearHashMap<V>, key: uint64)
+  returns (linear removed: lOption<V>)
+  requires FixedSizeInv(old_self)
+  ensures IsFixedSizeRemove(old_self, key, self, removed)
+  ensures FixedSizeInv(self)
+  {
+    var slotIdx := Probe(self, key);
+    var _ := LemmaProbeResult(self, key);
+
+    if lseq_peek(self.storage, slotIdx).Entry? {
+      linear var item: lItem<V> := lseq_take_inout(inout self.storage, slotIdx);
+      lseq_give_inout(inout self.storage, slotIdx, lItem.Tombstone(key));
+      linear var Entry(_, value) := item;
+      removed := lSome(value);
+
+      inout ghost self.contents := self.contents[key := None];
+      assert EntryInSlotMatchesContents(toItems(old_self.storage), Slot(slotIdx as int), old_self.contents);
+    } else {
+      removed := lNone;
+    }
+    LemmaFixedSizeRemove(old_self, key, self, removed);
+  }
+
+  lemma LemmaFixedSizeRemove<V>(self: FixedSizeLinearHashMap<V>, key: uint64, 
+    self': FixedSizeLinearHashMap<V>, removed: lOption<V>)
+  requires IsFixedSizeRemove.requires(self, key, self', removed)
+  requires IsFixedSizeRemove(self, key, self', removed)
+  ensures FixedSizeInv(self')
+  {
+    var probeRes := LemmaProbeResult(self, key);
+    var slotIdx := probeRes.slotIdx;
+    var probeStartSlotIdx := probeRes.startSlotIdx;
+    var probeSkips := probeRes.ghostSkips;
+
+    if self.storage[slotIdx as nat].Entry? {
+      forall explainedKey | explainedKey in self'.contents
+      ensures exists skips :: SlotExplainsKey(toItems(self'.storage), skips, explainedKey)
+      {
+        if key == explainedKey {
+          assert SlotExplainsKey(toItems(self'.storage), probeSkips as nat, key);
+        } else {
+          var oldSkips :| SlotExplainsKey(toItems(self.storage), oldSkips, explainedKey);
+          assert SlotExplainsKey(toItems(self'.storage), oldSkips, explainedKey);
+        }
+      }
+
+      forall slot | ValidSlot(|self'.storage|, slot) && toItems(self'.storage)[slot.slot].Entry?
+      ensures && var item := self'.storage[slot.slot];
+              && self'.contents[item.key] == Some(item.value)
+      {
+        var item := self'.storage[slot.slot];
+        if slot != Slot(slotIdx as nat) && item.key == key {
+          assert CantEquivocateStorageKey(toItems(self'.storage));
+          assert TwoNonEmptyValidSlotsWithSameKey(toItems(self'.storage), slot, Slot(slotIdx as nat));
+          assert false;
+        }
+      }
+    }
+  }
+
+  //////// Resizing Hash Map
+
+  linear datatype LinearHashMap<V> = LinearHashMap(
+    linear underlying: FixedSizeLinearHashMap<V>,
+    count: uint64,
+    ghost contents: map<uint64, V>)
+  {
+    predicate Inv() {Inv0(this)} // HACK Inv0: is there a better way to refer to the outer Inv(...) from inside Inv()?
+  }
+
+  lemma CantEquivocateMapFromStorageKey<V>(underlying: FixedSizeLinearHashMap<V>)
+  requires FixedSizeInv(underlying)
+  ensures CantEquivocate(toItems(underlying.storage))
+  {
+    assert |underlying.storage| > 0;
+    assert ValidSlot(|underlying.storage|, Slot(0));
+    assert exists slot :: ValidSlot(|underlying.storage|, slot);
+    forall slot1, slot2 | (
+      && ValidSlot(|underlying.storage|, slot1) && ValidSlot(|underlying.storage|, slot2)
+      && underlying.storage[slot1.slot].Entry? && underlying.storage[slot2.slot].Entry?
+      && underlying.storage[slot1.slot].key == underlying.storage[slot2.slot].key)
+    ensures slot1 == slot2
+    {
+      assert CantEquivocateStorageKey(toItems(underlying.storage));
+      if underlying.storage[slot1.slot].Entry? && underlying.storage[slot2.slot].Entry? &&
+        underlying.storage[slot1.slot].key == underlying.storage[slot2.slot].key {
+
+        assert TwoNonEmptyValidSlotsWithSameKey(toItems(underlying.storage), slot1, slot2);
+        if slot1 != slot2 {
+          assert false;
+        }
+        assert slot1 == slot2;
+      } else {
+        assert slot1 == slot2;
+      }
+    }
+  }
+
+  predicate UnderlyingContentsMatchesContents<V>(underlying: FixedSizeLinearHashMap<V>, contents: map<uint64, V>)
+  {
+    && (forall key :: key in contents ==> key in underlying.contents && underlying.contents[key] == Some(contents[key]))
+    && (forall key :: key !in contents ==> key !in underlying.contents || underlying.contents[key].None?)
+  }
+
+  predicate UnderlyingInv<V>(self: LinearHashMap<V>, underlying: FixedSizeLinearHashMap<V>)
+  {
+    && |self.contents| == self.count as nat
+    && UnderlyingContentsMatchesContents(underlying, self.contents)
+    && FixedSizeInv(underlying)
+    && MapFromStorage(toItems(underlying.storage)) == self.contents
+  }
+
+  lemma UnderlyingInvImpliesMapFromStorageMatchesContents<V>(underlying: FixedSizeLinearHashMap<V>, contents: map<uint64, V>)
+  requires UnderlyingContentsMatchesContents(underlying, contents)
+  requires FixedSizeInv(underlying)
+  ensures MapFromStorage(toItems(underlying.storage)) == contents
+  {
+    var mapFromStorage := MapFromStorage(toItems(underlying.storage));
+    CantEquivocateMapFromStorageKey(underlying);
+    MapFromStorageProperties(toItems(underlying.storage), mapFromStorage);
+    assert MapFromStorage(toItems(underlying.storage)) == contents;
+  }
+
+  predicate Inv0<V>(self: LinearHashMap<V>) { Inv(self) }
+
+  protected predicate Inv<V>(self: LinearHashMap<V>)
+  ensures Inv(self) ==> |self.contents| == self.count as nat
+  ensures Inv(self) ==> UnderlyingInv(self, self.underlying)
+  {
+    && UnderlyingInv(self, self.underlying)
+    && MapFromStorage(toItems(self.underlying.storage)) == self.contents
+    && |self.contents| == self.count as nat
+    && (self.count as nat) <= 0x1_0000_0000_0000_0000 / 8
+  }
+
+  lemma CountBound<V>(self: LinearHashMap<V>)
+  requires Inv(self)
+  ensures self.count as int <= 0x1_0000_0000_0000_0000 / 8
+  {
+  }
+
+  lemma RevealProtectedInv<V>(self: LinearHashMap<V>)
+    requires Inv(self)
+    ensures (
+      && UnderlyingInv(self, self.underlying)
+      && MapFromStorage(toItems(self.underlying.storage)) == self.contents
+      && |self.contents| == self.count as nat)
+  {
+  }
+
+  predicate IsConstructor<V>(self: LinearHashMap<V>, size: uint64)
+  requires 128 <= size
+  {
+    && Inv(self)
+    && self.contents == map[]
+  }
+
+  method Constructor<V>(size: uint64) returns (linear self: LinearHashMap<V>)
+  requires 128 <= size
+  ensures IsConstructor(self, size)
+  {
+    linear var fixed := ConstructorFromSize(size);
+    self := LinearHashMap(fixed, 0, map[]);
+
+    assert forall slot :: ValidSlot(|self.underlying.storage|, slot) ==> !self.underlying.storage[slot.slot].Entry?;
+    UnderlyingInvImpliesMapFromStorageMatchesContents(self.underlying, self.contents);
+    assert MapFromStorage(toItems(self.underlying.storage)) == self.contents;
+  }
+
+  lemma LemmaEntryKeyInContents<V>(self: LinearHashMap<V>, i: uint64)
+  requires Inv(self)
+  requires 0 <= i as int < |self.underlying.storage|
+  requires self.underlying.storage[i as nat].Entry?
+  ensures self.underlying.storage[i as nat].key in self.contents
+  {
+    assert EntryInSlotMatchesContents(toItems(self.underlying.storage), Slot(i as nat), self.underlying.contents); // trigger
+  }
+
+  predicate IsRealloc<V>(self: LinearHashMap<V>, self': LinearHashMap<V>)
+  requires Inv(self)
+  requires self.count as nat < 0x1_0000_0000_0000_0000 / 8
+  {
+    && self'.contents == self.contents
+    && self'.underlying.count as nat < |self'.underlying.storage| - 2
+    && Inv(self')
+  }
+
+  method Realloc<V>(linear inout self: LinearHashMap<V>)
+  requires Inv(old_self)
+  requires old_self.count as nat < 0x1_0000_0000_0000_0000 / 8
+  ensures IsRealloc(old_self, self)
+  {
+    var newSize: uint64 := (128 + self.count) * 4;
+    linear var newUnderlying := ConstructorFromSize(newSize);
+
+    ghost var transferredContents := map[];
+    ghost var transfers := toItems(self.underlying.storage);
+    CantEquivocateMapFromStorageKey(self.underlying);
+
+    var i := 0 as uint64;
+    var size := lseq_length_as_uint64(self.underlying.storage);
+
+    while i < size
+      invariant i <= size
+      invariant size as nat == |self.underlying.storage|
+      invariant self.count as nat == |self.contents|
+      invariant |newUnderlying.storage| == newSize as nat
+
+      invariant transferredContents.Keys <= self.contents.Keys
+      invariant newUnderlying.count as nat == |transferredContents|
+      invariant newUnderlying.count as nat < |newUnderlying.storage| - 2
+      invariant (forall key :: key in newUnderlying.contents ==> 
+        EntryExistsInElements(transfers, i, key))
+
+      invariant FixedSizeInv(newUnderlying)
+      invariant UnderlyingContentsMatchesContents(newUnderlying, transferredContents)
+      invariant toItems(self.underlying.storage)[i..] == transfers[i..]
+      invariant MapFromStorage(transfers[..i]) == transferredContents
+      invariant MapFromStorage(transfers) == self.contents
+
+      invariant (forall j | i as nat <= j < size as nat :: lseq_has(self.underlying.storage)[j])
+      invariant (forall j | 0 <= j < i as nat :: !lseq_has(self.underlying.storage)[j])
+    {
+      assert i < size;
+      assert Last(transfers[..i+1]) == transfers[i];
+      assert transfers[..i] == DropLast(transfers[..i+1]);
+
+      linear var item := lseq_take_inout(inout self.underlying.storage, i);
+      if item.Entry? {
+        ElementsEntryInMap(transfers, item.toItem());
+        if item.key in newUnderlying.contents {
+          var j:uint64 :| (
+              && 0 <= j < i
+              && ValidSlot(|transfers|, Slot(j as int))
+              && transfers[Slot(j as int).slot].Entry?
+              && transfers[Slot(j as int).slot].key == item.key);
+          assert ValidSlot(|transfers|, Slot(i as nat));
+          assert false;
+        }
+        assert item.key !in newUnderlying.contents;
+
+        assert transferredContents.Keys <= self.contents.Keys;
+        SetInclusionImpliesSmallerCardinality(transferredContents.Keys, self.contents.Keys);
+        assert |transferredContents.Keys| <= |self.contents.Keys|;
+        assert |transferredContents| <= |self.contents|;
+        assert newUnderlying.count as nat < |newUnderlying.storage| - 1;
+
+        // ------ Mutation ------
+        transferredContents := transferredContents[item.key := item.value];
+        linear var replaced := FixedSizeInsertEntry(inout newUnderlying, item);
+        // ----------------------
+        linear match replaced { case lNone() => }
+        assert ValidSlot(|transfers|, Slot(i as nat));
+        assert FixedSizeInv(newUnderlying);
+      } else {
+        item.FreeNonEntry();
+      }
+      assert newUnderlying.count as nat < |newUnderlying.storage| - 2;
+      i := i + 1;
+    }
+
+    assert transfers[..i] == transfers;
+    assert UnderlyingContentsMatchesContents(newUnderlying, transferredContents);
+    assert UnderlyingContentsMatchesContents(newUnderlying, self.contents);
+    UnderlyingInvImpliesMapFromStorageMatchesContents(newUnderlying, self.contents);
+
+    linear var oldUnderlying := Replace(inout self.underlying, newUnderlying);
+    linear var FixedSizeLinearHashMap(oldstorage, _, _) := oldUnderlying;
+    lseq_free(oldstorage);
+  }
+
+  method Insert<V>(linear inout self: LinearHashMap, key: uint64, linear value: V) 
+  returns (linear replaced: lOption<V>)
+  requires Inv(old_self)
+  requires old_self.count as nat < 0x1_0000_0000_0000_0000 / 8
+  ensures
+    && Inv(self)
+    && self.contents == old_self.contents[key := value]
+    && self.count as nat == old_self.count as nat + (if replaced.lSome? then 0 else 1)
+    && (replaced.lSome? ==> MapsTo(old_self.contents, key, replaced.value))
+    && (replaced.lNone? ==> key !in old_self.contents)
+  {
+    var len := lseq_length_as_uint64(self.underlying.storage);
+    if len / 2 <= self.underlying.count {
+      Realloc(inout self);
+    }
+    // --------------
+
+    // -- mutation --
+    replaced := FixedSizeInsert(inout self.underlying, key, value);
+    inout ghost self.contents := self.contents[key := value];
+    if replaced.lNone? {
+      inout self.count := self.count + 1;
+    }
+    // --------------
+
+    UnderlyingInvImpliesMapFromStorageMatchesContents(self.underlying, self.contents);
+  }
+
+  method Remove<V>(linear inout self: LinearHashMap, key: uint64) 
+  returns (linear removed: lOption<V>)
+  requires Inv(old_self)
+  ensures Inv(self)
+  ensures removed.lSome? ==>
+      key in old_self.contents && old_self.contents[key] == removed.value
+  ensures removed.lNone? ==> key !in old_self.contents
+  ensures (self.contents == if key in old_self.contents
+      then map k | k in old_self.contents && k != key :: old_self.contents[k]
+      else old_self.contents)
+  {
+    // -- mutation --
+    removed := FixedSizeRemove(inout self.underlying, key);
+    inout ghost self.contents := map k | k in self.contents && k != key :: self.contents[k];
+    if removed.lSome? {
+      inout self.count := self.count - 1;
+    }
+    // -------------- 
+
+    UnderlyingInvImpliesMapFromStorageMatchesContents(self.underlying, self.contents); 
+    assert self.count as nat == |self.contents| by {
+      if removed.lSome? {
+        assert key in old_self.contents;
+        assert self.contents.Keys <= old_self.contents.Keys;
+        assert |old_self.contents| == self.count as nat + 1;
+        assert |old_self.contents.Keys| == self.count as nat + 1;
+        assert |old_self.contents.Keys - {key}| == |old_self.contents.Keys| - |{key}|;
+        assert old_self.contents.Keys - {key} == self.contents.Keys;
+        assert |self.contents| == |old_self.contents| - 1;
+        assert |self.contents| == self.count as nat;
+      } else {
+        assert key !in old_self.contents;
+        assert self.contents == old_self.contents;
+        assert |self.contents| == self.count as nat;
+      }
+    }
+  }
+
+  method Get<V>(shared self: LinearHashMap, key: uint64) returns (shared result: V)
+  requires Inv(self)
+  requires IsEntry(self.underlying, key)
+  ensures key in self.contents && result == self.contents[key]
+  {
+    result := FixedSizeGet(self.underlying, key);
+    LemmaFixedSizeGet(self.underlying, key);
+  }
+
+  //////// Iterator
+
+  // We have two types of iterators.
+  //
+  // Iterator is usually more convenient as it has the IteratorOutput
+  // built-in.
+  //
+  // SimpleIterator doesn't (you have to call SimpleIteratorOutput)
+  // but has the advantage that the WFSimpleIter condition doesn't
+  // depend on the key/value being correct. Thus the well-formedness
+  // of a SimpleIterator can be preserved across (some) modifications
+  // of the hash map.
+  //
+  // TODO fix the duplicated code that results.
+
+  datatype IteratorOutput<V> = Next(key: uint64) | Done
+
+  datatype Iterator<V> = Iterator(
+    i: uint64, // index in hash table item list
+    ghost s: set<uint64>,   // set of values returned so far
+    ghost decreaser: ORDINAL,
+    next: IteratorOutput)
+
+  datatype SimpleIterator = SimpleIterator(
+    i: uint64, // index in hash table item list
+    ghost s: set<uint64>,   // set of values returned so far
+    ghost decreaser: ORDINAL)
+
+  predicate NextExplainedByI<V>(self: LinearHashMap<V>, i : uint64, output:IteratorOutput)
+  {
+    && (output.Next? ==>
+      && i as int < |self.underlying.storage|
+      && self.underlying.storage[i as nat].Entry?
+      && self.underlying.storage[i as nat].key == output.key)
+    && (output.Done? ==> i as int == |self.underlying.storage|)
+  }
+
+  predicate ValidI<V>(self: LinearHashMap<V>, it: Iterator<V>)
+  {
+    && 0 <= it.i as int <= |self.underlying.storage|
+  }
+
+  predicate EachReturnedKeyExplainedByPassedIndex<V>(self: LinearHashMap<V>, s: set<uint64>, i: uint64)
+  requires 0 <= i as int <= |self.underlying.storage|
+  {
+    forall key | key in s ::
+        exists j | 0 <= j < i as int ::
+        && self.underlying.storage[j].Entry?
+        && key == self.underlying.storage[j].key
+  }
+
+  protected predicate WFIter<V>(self: LinearHashMap<V>, it: Iterator<V>)
+  ensures WFIter(self, it) ==> (it.next.Done? ==> it.s == self.contents.Keys)
+  ensures WFIter(self, it) ==> (it.next.Next? ==> it.next.key in self.contents)
+  ensures WFIter(self, it) ==> (it.next.Next? ==> it.next.key !in it.s)
+  ensures WFIter(self, it) ==> it.s <= self.contents.Keys
+  {
+    && ValidI(self, it)
+    && NextExplainedByI(self, it.i, it.next)
+    // Done justified by exhausting i
+    && (it.next.Done? ==> (it.s == self.contents.Keys))
+    // Each passed index appears in s
+    && (forall j | 0 <= j < it.i as int ::
+        self.underlying.storage[j].Entry? ==> self.underlying.storage[j].key in it.s)
+    && EachReturnedKeyExplainedByPassedIndex(self, it.s, it.i)
+    && it.decreaser == (|self.underlying.storage| - it.i as int) as ORDINAL
+    && (it.next.Next? ==> it.next.key in self.contents)
+    && (it.next.Next? ==> it.next.key !in it.s)
+    && it.s <= self.contents.Keys
+  }
+
+  protected predicate WFSimpleIter<V>(self: LinearHashMap<V>, it: SimpleIterator)
+  ensures WFSimpleIter(self, it) ==> it.s <= self.contents.Keys
+  {
+    && 0 <= it.i as int <= |self.underlying.storage| < Uint64UpperBound()
+    && (it.i as int == |self.underlying.storage| ==> (it.s == self.contents.Keys))
+    && (it.i as int < |self.underlying.storage| ==> self.underlying.storage[it.i as nat].Entry?)
+    // Each passed index appears in s
+    && (forall j | 0 <= j < it.i as int ::
+        self.underlying.storage[j].Entry? ==> self.underlying.storage[j].key in it.s)
+    && EachReturnedKeyExplainedByPassedIndex(self, it.s, it.i)
+    && it.decreaser == (|self.underlying.storage| - it.i as int) as ORDINAL
+    && (it.i as int < |self.underlying.storage| ==> (
+      && self.underlying.storage[it.i as nat].key in self.contents
+      && self.underlying.storage[it.i as nat].key !in it.s
+    ))
+    && it.s <= self.contents.Keys
+  }
+
+  function method indexOutput<V>(shared self: LinearHashMap<V>, i: uint64) : (next: IteratorOutput<V>)
+  requires Inv(self)
+  requires 0 <= i as int <= |self.underlying.storage| < Uint64UpperBound()
+  requires i as int < |self.underlying.storage| ==> self.underlying.storage[i as nat].Entry?
+  {
+    if i == lseq_length_as_uint64(self.underlying.storage) then (
+      Done
+    ) else (
+      Next(lseq_peek(self.underlying.storage, i).key)
+    )
+  }
+
+  protected function method SimpleIterOutput<V>(shared self: LinearHashMap<V>, it: SimpleIterator) : (next: IteratorOutput<V>)
+  requires Inv(self)
+  requires WFSimpleIter(self, it)
+  ensures (next.Done? ==> it.s == self.contents.Keys)
+  ensures (next.Next? ==> next.key in self.contents)
+  ensures (next.Next? ==> next.key !in it.s)
+  {
+    indexOutput(self, it.i)
+  }
+
+  lemma LemmaWFIterImpliesILt<V>(self: LinearHashMap<V>, it: Iterator<V>)
+  requires WFIter(self, it)
+  ensures it.next.Next? ==> it.i as int < |self.underlying.storage|
+  {
+  }
+
+  lemma LemmaWFSimpleIterImpliesEntry<V>(self: LinearHashMap<V>, it: SimpleIterator)
+  requires Inv(self)
+  requires WFSimpleIter(self, it)
+  ensures
+    && 0 <= it.i as int <= |self.underlying.storage|
+    && (SimpleIterOutput(self, it).Next? ==> it.i as int < |self.underlying.storage|)
+    && (it.i as int < |self.underlying.storage| ==>
+      && self.underlying.storage[it.i as nat].Entry?
+    )
+  {
+  }
+
+  lemma LemmaIterNextNotInS<V>(self: LinearHashMap<V>, it: Iterator<V>)
+  requires 0 <= it.i as int <= |self.underlying.storage|
+  requires ValidElements(toItems(self.underlying.storage))
+  requires CantEquivocateStorageKey(toItems(self.underlying.storage))
+  requires NextExplainedByI(self, it.i, it.next)
+  requires EachReturnedKeyExplainedByPassedIndex(self, it.s, it.i)
+  ensures (it.next.Next? ==> it.next.key !in it.s)
+  {
+    if it.next.Next? {
+      if it.next.key in it.s {
+        var j :| 0 <= j < it.i as int
+          && self.underlying.storage[j].Entry?
+          && it.next.key == self.underlying.storage[j].key;
+        assert TwoNonEmptyValidSlotsWithSameKey<V>(toItems(self.underlying.storage), Slot(it.i as int), Slot(j));  // trigger
+        assert false; // proof by contradiction
+      }
+    }
+  }
+
+  function method iterToNext<V>(shared self: LinearHashMap<V>, i: uint64) : (res: (uint64, IteratorOutput))
+  requires Inv(self)
+  requires 0 <= i as int <= |self.underlying.storage|
+  ensures NextExplainedByI(self, res.0, res.1)
+  ensures forall j | i <= j < res.0 :: !self.underlying.storage[j as nat].Entry?
+  ensures i <= res.0
+  decreases |self.underlying.storage| - i as int
+  {
+    if i == lseq_length_as_uint64(self.underlying.storage) then (
+      (i, Done)
+    ) else if lseq_peek(self.underlying.storage, i).Entry? then (
+      (i, Next(lseq_peek(self.underlying.storage, i).key))
+    ) else (
+      iterToNext(self, i+1)
+    )
+  }
+
+  function method simpleIterToNext<V>(shared self: LinearHashMap<V>, i: uint64) : (i': uint64)
+  requires Inv(self)
+  requires 0 <= i as int <= |self.underlying.storage|
+  ensures 0 <= i' as int <= |self.underlying.storage|
+  ensures forall j | i <= j < i' :: !self.underlying.storage[j as nat].Entry?
+  ensures i' as int < |self.underlying.storage| ==>
+      self.underlying.storage[i' as nat].Entry?
+  ensures i <= i'
+  decreases |self.underlying.storage| - i as int
+  {
+    if i == lseq_length_as_uint64(self.underlying.storage) then (
+      i
+    ) else if lseq_peek(self.underlying.storage, i).Entry? then (
+      i
+    ) else (
+      simpleIterToNext(self, i+1)
+    )
+  }
+
+  lemma lemmaIterToNextValidKey<V>(self: LinearHashMap<V>, i: uint64)
+  requires Inv(self)
+  requires 0 <= i as int <= |self.underlying.storage|
+  ensures iterToNext(self, i).1.Next? ==> iterToNext(self, i).1.key in self.contents
+  {
+    var j := iterToNext(self, i).0;
+    var next := iterToNext(self, i).1;
+    if next.Next? {
+      UnderlyingInvImpliesMapFromStorageMatchesContents(self.underlying, self.contents);
+      CantEquivocateMapFromStorageKey(self.underlying);
+      MapFromStorageProperties(toItems(self.underlying.storage), self.contents);
+      assert self.underlying.storage[Slot(j as int).slot].key == next.key; // trigger
+    }
+  }
+
+  function method {:opaque} IterStart<V>(shared self: LinearHashMap<V>) : (it' : Iterator<V>)
+  requires Inv(self)
+  ensures WFIter(self, it')
+  ensures it'.s == {}
+  {
+    lemmaIterToNextValidKey(self, 0);
+
+    var (i, next) := iterToNext(self, 0);
+    var it' := Iterator(i, {}, (|self.underlying.storage| - i as int) as ORDINAL, next);
+
+    LemmaIterNextNotInS(self, it');
+
+    it'
+  }
+
+  function method {:opaque} SimpleIterStart<V>(shared self: LinearHashMap<V>) : (it' : SimpleIterator)
+  requires Inv(self)
+  ensures WFSimpleIter(self, it')
+  ensures it'.s == {}
+  {
+    lemmaIterToNextValidKey(self, 0);
+
+    var i := simpleIterToNext(self, 0);
+    var it' := SimpleIterator(i, {}, (|self.underlying.storage| - i as int) as ORDINAL);
+
+    LemmaIterNextNotInS(self,
+      Iterator(it'.i, it'.s, it'.decreaser, indexOutput(self, it'.i)));
+
+    it'
+  }
+
+  function method {:opaque} IterInc<V>(shared self: LinearHashMap<V>, it: Iterator) : (it' : Iterator)
+  requires Inv(self)
+  requires WFIter(self, it)
+  requires it.next.Next?
+  ensures WFIter(self, it')
+  ensures it'.s == it.s + {it.next.key}
+  ensures it'.next.Done? ==> it'.s == self.contents.Keys
+  ensures it'.decreaser < it.decreaser
+  {
+    lemmaIterToNextValidKey(self, it.i + 1);
+
+    var (i, next) := iterToNext(self, it.i + 1);
+    var it' := Iterator(i, it.s + {it.next.key}, (|self.underlying.storage| - i as int) as ORDINAL, next);
+
+    assert (forall key | key in it'.s ::
+        exists j | 0 <= j < it'.i as int ::
+        && self.underlying.storage[j].Entry?
+        && key == self.underlying.storage[j].key);
+    assert (it'.next.Done? ==> it'.s == self.contents.Keys);
+
+    LemmaIterNextNotInS(self, it');
+
+    it'
+  }
+
+  function method {:opaque} SimpleIterInc<V>(shared self: LinearHashMap<V>, it: SimpleIterator) : (it' : SimpleIterator)
+  requires Inv(self)
+  requires WFSimpleIter(self, it)
+  requires SimpleIterOutput(self, it).Next?
+  ensures WFSimpleIter(self, it')
+  ensures it'.s == it.s + {SimpleIterOutput(self, it).key}
+  ensures it'.decreaser < it.decreaser
+  {
+    lemmaIterToNextValidKey(self, it.i + 1);
+
+    var i := simpleIterToNext(self, it.i + 1);
+    var it' := SimpleIterator(i, it.s + {SimpleIterOutput(self, it).key}, (|self.underlying.storage| - i as int) as ORDINAL);
+
+    assert (forall key | key in it'.s ::
+        exists j | 0 <= j < it'.i as int ::
+        && self.underlying.storage[j].Entry?
+        && key == self.underlying.storage[j].key);
+
+    LemmaIterNextNotInS(self,
+      Iterator(it'.i, it'.s, it'.decreaser, indexOutput(self, it'.i)));
+
+    it'
+  }
+
+  lemma LemmaIterIndexLtCount<V>(self: LinearHashMap<V>, it: Iterator<V>)
+  requires Inv(self)
+  requires WFIter(self, it)
+  ensures it.next.Next? ==> |it.s| < self.count as int
+  {
+    if it.next.Next? {
+      ProperSubsetImpliesSmallerCardinality(it.s, self.contents.Keys);
+    }
+  }
+
+  function method MaxKeyIterate<V>(shared self: LinearHashMap<V>, it: Iterator<V>, m: uint64) : (res : uint64)
+  requires Inv(self)
+  requires WFIter(self, it)
+  requires forall key | key in it.s :: key <= m
+  ensures forall key | key in self.contents :: key <= res
+  decreases it.decreaser
+  {
+    if it.next.Done? then (
+      m
+    ) else (
+      var key := it.next.key;
+      MaxKeyIterate(self, IterInc(self, it), if m < key then key else m)
+    )
+  }
+
+  function method {:opaque} MaxKey<V>(shared self: LinearHashMap<V>) : (res : uint64)
+  requires Inv(self)
+  ensures forall key | key in self.contents :: key <= res
+  {
+    MaxKeyIterate(self, IterStart(self), 0)    
+  }
+
+  predicate IsUpdateByIter<V>(self: LinearHashMap<V>, it: SimpleIterator, value: V, 
+    self': LinearHashMap<V>, replaced: V)
+  requires Inv(self)
+  requires WFSimpleIter(self, it)
+  requires SimpleIterOutput(self, it).Next?
+  {
+    && self.count == self'.count
+    && self'.contents == self.contents[SimpleIterOutput(self, it).key := value]
+    && IsFixedSizeUpdateBySlot(self.underlying, it.i, value, self'.underlying, replaced)
+  }
+
+  method UpdateByIter<V>(linear inout self: LinearHashMap<V>, it: SimpleIterator, linear value: V) 
+  returns (linear replaced: V)
+  requires Inv(old_self)
+  requires WFSimpleIter(old_self, it)
+  requires SimpleIterOutput(old_self, it).Next?
+  ensures Inv(self)
+  ensures self.contents == old_self.contents[SimpleIterOutput(old_self, it).key := value]
+  ensures self.count == old_self.count
+  ensures IsUpdateByIter(old_self, it, value, self, replaced)
+  {
+    inout ghost self.contents := self.contents[SimpleIterOutput(self, it).key := value];
+    replaced := FixedSizeUpdateBySlot(inout self.underlying, it.i, value);
+
+    UnderlyingInvImpliesMapFromStorageMatchesContents(self.underlying, self.contents);
+  }
+
+  function setUpTo<V>(self: LinearHashMap<V>, i: int) : set<uint64>
+  requires 0 <= i <= |self.underlying.storage|
+  {
+    set j | 0 <= j < i && self.underlying.storage[j].Entry?
+        :: self.underlying.storage[j].key
+  }
+
+  lemma setUpToLeContents<V>(self: LinearHashMap<V>, i: int)
+  requires Inv(self)
+  requires 0 <= i <= |self.underlying.storage|
+  ensures setUpTo(self, i) <= self.contents.Keys
+  {
+    forall j | 0 <= j < i && self.underlying.storage[j].Entry?
+    ensures self.underlying.storage[j].key in self.contents
+    {
+      var key := self.underlying.storage[j].key;
+      var slot := Slot(j);
+      assert ValidSlot(|self.underlying.storage|, slot);
+      CantEquivocateMapFromStorageKey(self.underlying);
+      MapFromStorageProperties(toItems(self.underlying.storage), self.contents);
+    }
+  }
+
+  function method {:opaque} FindSimpleIter<V>(shared self: LinearHashMap<V>, key: uint64)
+    : (it : SimpleIterator)
+  requires Inv(self)
+  ensures WFSimpleIter(self, it)
+  ensures key in self.contents ==> SimpleIterOutput(self, it) == Next(key)
+  ensures key !in self.contents ==> SimpleIterOutput(self, it) == Done
+  {
+    var idx := Probe(self.underlying, key);
+
+    var i := if lseq_peek(self.underlying.storage, idx).Entry? then idx
+      else lseq_length_as_uint64(self.underlying.storage) as uint64;
+    var it := SimpleIterator(i, setUpTo(self, i as int), (|self.underlying.storage| - i as int) as ORDINAL);
+
+    assert WFSimpleIter(self, it)
+      && (key in self.contents ==>
+        SimpleIterOutput(self, it) == Next(key))
+      && (key !in self.contents ==>
+        SimpleIterOutput(self, it) == Done)
+    by {
+      var result := LemmaProbeResult(self.underlying, key);
+      if it.i as int < |self.underlying.storage| {
+        if self.underlying.storage[it.i as nat].key in it.s {
+          var j :| 0 <= j < it.i && self.underlying.storage[j as nat].Entry?
+              && self.underlying.storage[j as nat].key == key;
+          assert TwoNonEmptyValidSlotsWithSameKey(
+              toItems(self.underlying.storage), Slot(j as int), Slot(it.i as int));
+        }
+      }
+      setUpToLeContents(self, i as int);
+    }
+  
+    it
+  }
+}
